per/sequents_ext.v
@@ -1,0 +1,215 @@
+(*
+
+  Copyright 2014 Cornell University
+  Copyright 2015 Cornell University
+  Copyright 2016 Cornell University
+  Copyright 2017 Cornell University
+
+  This file is part of VPrl (the Verified Nuprl project).
+
+  VPrl is free software: you can redistribute it and/or modify
+  it under the terms of the GNU General Public License as published by
+  the Free Software Foundation, either version 3 of the License, or
+  (at your option) any later version.
+
+  VPrl is distributed in the hope that it will be useful,
+  but WITHOUT ANY WARRANTY; without even the implied warranty of
+  MERCHANTABILITY or FITNESS FOR A PARTICULAR PURPOSE.  See the
+  GNU General Public License for more details.
+
+  You should have received a copy of the GNU General Public License
+  along with VPrl.  If not, see <http://www.gnu.org/licenses/>.
+
+
+  Websites: http://nuprl.org/html/verification/
+            http://nuprl.org/html/Nuprl2Coq
+            https://github.com/vrahli/NuprlInCoq
+
+  Authors: Vincent Rahli
+
+*)
+
+
+Require Export sequents.
+
+
+Definition ext_sequent_true {o} lib (S : @csequent o) : Type :=
+  forall s1 s2,
+    match destruct_csequent S with
+    | cseq_comps H T wh wt ct ec =>
+      forall p : similarity lib s1 s2 H,
+        match ec with
+        | Some (existT _ ext (we, ce)) =>
+          equality
+            lib
+            (lsubstc ext we s1 (s_cover_ex1 lib ext s1 s2 H ce p))
+            (lsubstc ext we s2 (s_cover_ex2 lib ext s1 s2 H ce p))
+            (lsubstc T wt s1 (s_cover_typ1 lib T s1 s2 H ct p))
+          /\
+          equality
+            lib
+            (lsubstc ext we s1 (s_cover_ex1 lib ext s1 s2 H ce p))
+            (lsubstc ext we s2 (s_cover_ex2 lib ext s1 s2 H ce p))
+            (lsubstc T wt s2 (s_cover_typ2 lib T s1 s2 H ct p))
+        | None => True
+        end
+    end.
+
+Definition ext_rule_true {o} lib (R : @rule o) : Type :=
+  forall (wg : wf_sequent (goal R))
+         (cg : closed_type_baresequent (goal R))
+         (cargs: args_constraints (sargs R) (hyps (goal R)))
+         (hyps :
+            forall s : baresequent,
+              LIn s (subgoals R)
+              -> {c : wf_csequent s & ext_sequent_true lib (mk_wcseq s c)}),
+    {c : closed_extract_baresequent (goal R)
+     & ext_sequent_true lib (mk_wcseq (goal R) (ext_wf_cseq (goal R) wg cg c))}.
+Hint Unfold ext_rule_true.
+
+Lemma ext_sequent_true_all {o} :
+  forall lib (S : @csequent o),
+    ext_sequent_true lib S
+    <=>
+    forall s1 s2,
+      match destruct_csequent S with
+        | cseq_comps H T wh wt ct ec =>
+            forall (pC1 : cover_vars T s1) (pC2 : cover_vars T s2),
+              similarity lib s1 s2 H
+              -> match ec with
+                   | Some (existT _ ext (we, ce)) =>
+                       forall (pt1 : cover_vars ext s1) (pt2 : cover_vars ext s2),
+                         equality
+                           lib
+                           (lsubstc ext we s1 pt1)
+                           (lsubstc ext we s2 pt2)
+                           (lsubstc T wt s1 pC1)
+                         /\
+                         equality
+                           lib
+                           (lsubstc ext we s1 pt1)
+                           (lsubstc ext we s2 pt2)
+                           (lsubstc T wt s2 pC2)
+                   | None => True
+                 end
+      end.
+Proof.
+  unfold ext_sequent_true; split; intro h;
+    destruct (destruct_csequent S); destruct ec; exrepnd; tcsp; introv;
+      try (complete (apply h; auto)).
+
+  introv sim; introv.
+  pose proof (h s2 s3 sim) as h; repnd.
+
+  rewrite lsubstc_replace with (w2 := wt) (p2 := pC1) in h0; auto.
+  rewrite lsubstc_replace with (w2 := wt) (p2 := pC2) in h; auto.
+  rewrite lsubstc_replace with (w2 := s1) (p2 := pt1) in h0; auto.
+  rewrite lsubstc_replace with (w2 := s1) (p2 := pt1) in h; auto.
+  rewrite lsubstc_replace with (w2 := s1) (p2 := pt2) in h0; auto.
+  rewrite lsubstc_replace with (w2 := s1) (p2 := pt2) in h; auto.
+Qed.
+
+Lemma ext_sequent_true_ex {o} :
+  forall lib (S : @csequent o),
+    ext_sequent_true lib S
+    <=>
+    forall s1 s2,
+      match destruct_csequent S with
+        | cseq_comps H T wh wt ct ec =>
+          similarity lib s1 s2 H
+          -> {pC1 : cover_vars T s1
+              & {pC2 : cover_vars T s2
+              & match ec with
+                | Some (existT _ ext (we, ce)) =>
+                  {pt1 : cover_vars ext s1
+                   & {pt2 : cover_vars ext s2
+                   & equality
+                       lib
+                       (lsubstc ext we s1 pt1)
+                       (lsubstc ext we s2 pt2)
+                       (lsubstc T wt s1 pC1)
+                   # equality
+                       lib
+                       (lsubstc ext we s1 pt1)
+                       (lsubstc ext we s2 pt2)
+                       (lsubstc T wt s2 pC2)
+                  }}
+                | None => True
+                end
+             }}
+      end.
+Proof.
+  unfold ext_sequent_true; split; intro h; introv;
+    destruct (destruct_csequent S); destruct ec; exrepnd; tcsp; intro sim; auto.
+
+  {
+    pose proof (h s1 s2 sim) as q.
+
+    exists (s_cover_typ1 lib T s1 s2 hs ct sim)
+           (s_cover_typ2 lib T s1 s2 hs ct sim)
+           (s_cover_ex1 lib t s1 s2 hs s0 sim)
+           (s_cover_ex2 lib t s1 s2 hs s0 sim); sp.
+  }
+
+  {
+    exists (s_cover_typ1 lib T s1 s2 hs ct sim)
+           (s_cover_typ2 lib T s1 s2 hs ct sim); sp.
+  }
+
+  {
+    pose proof (h s1 s2 sim) as q; exrepnd.
+
+    rewrite lsubstc_replace with (w2 := wt) (p2 := pC1); auto.
+    rewrite lsubstc_replace with (w2 := wt) (p2 := pC2); auto.
+    rewrite lsubstc_replace with (w2 := s3) (p2 := pt1); auto.
+    rewrite lsubstc_replace with (w2 := s3) (p2 := pt2); auto.
+  }
+Qed.
+
+Tactic Notation "ext_seq_true" :=
+  rw @ext_sequent_true_all;
+  simpl;
+  introv sim;
+  introv;
+  proof_irr;
+  GC.
+
+ Ltac ext_seq_true_ltac H :=
+  trw_h ext_sequent_true_ex  H;
+  simpl in H.
+
+Tactic Notation "ext_seq_true" "in" ident(H) :=
+  ext_seq_true_ltac H.
+
+
+Definition sp_ext_sequent_true {o} lib (S : @csequent o) : Type :=
+  forall s1 s2,
+    match destruct_csequent S with
+    | cseq_comps H T wh wt ct ec =>
+      forall p : similarity lib s1 s2 H,
+        match ec with
+        | Some (existT _ ext (we, ce)) =>
+          equality
+            lib
+            (lsubstc ext we s1 (s_cover_ex1 lib ext s1 s2 H ce p))
+            (lsubstc ext we s2 (s_cover_ex2 lib ext s1 s2 H ce p))
+            (lsubstc T wt s1 (s_cover_typ1 lib T s1 s2 H ct p))
+        | None => True
+        end
+    end.
+
+Lemma ext_sequent_true_iff_sp {o} :
+  forall lib (s : @csequent o), ext_sequent_true lib s <=> sp_ext_sequent_true lib s.
+Proof.
+  introv; split; introv h; introv.
+
+  - pose proof (h s1 s2) as q.
+    destruct (destruct_csequent s); introv; destruct ec; auto.
+    pose proof (q p) as w; clear q.
+    destruct s0; destruct p0; tcsp.
+
+  - pose proof (h s1 s2) as q.
+    destruct (destruct_csequent s); introv; destruct ec; auto.
+    pose proof (q p) as w; clear q.
+    destruct s0; destruct p0; dands; auto.
+Abort.
