rules/rules_function_ext.v
@@ -1,0 +1,3221 @@
+(*
+
+  Copyright 2014 Cornell University
+  Copyright 2015 Cornell University
+  Copyright 2016 Cornell University
+  Copyright 2017 Cornell University
+
+  This file is part of VPrl (the Verified Nuprl project).
+
+  VPrl is free software: you can redistribute it and/or modify
+  it under the terms of the GNU General Public License as published by
+  the Free Software Foundation, either version 3 of the License, or
+  (at your option) any later version.
+
+  VPrl is distributed in the hope that it will be useful,
+  but WITHOUT ANY WARRANTY; without even the implied warranty of
+  MERCHANTABILITY or FITNESS FOR A PARTICULAR PURPOSE.  See the
+  GNU General Public License for more details.
+
+  You should have received a copy of the GNU General Public License
+  along with VPrl.  If not, see <http://www.gnu.org/licenses/>.
+
+
+  Websites: http://nuprl.org/html/verification/
+            http://nuprl.org/html/Nuprl2Coq
+            https://github.com/vrahli/NuprlInCoq
+
+  Authors: Vincent Rahli
+
+*)
+
+
+Require Export sequents2.
+Require Export sequents_tacs.
+Require Export sequents_tacs2.
+Require Export rules_useful.
+Require Export per_props_equality.
+Require Export per_props_function.
+Require Export sequents_equality.
+Require Export rules_tyfam.
+Require Export subst_tacs_aeq.
+Require Export cequiv_tacs.
+Require Export sequents_ext.
+
+
+(** printing |- $\vdash$ *)
+(** printing ->  $\rightarrow$ *)
+(* begin hide *)
+
+
+Hint Resolve wf_term_subst : slow.
+Hint Rewrite @nh_vars_hyps_app : slow.
+Hint Rewrite @nh_vars_hyps_snoc : slow.
+
+Lemma subset_free_vars_csub_app3 {o} :
+  forall (t : @NTerm o) sub1 sub2,
+    disjoint (remove_nvars (dom_csub sub1) (free_vars t)) (dom_csub sub2)
+    -> csubst t (sub1 ++ sub2) = csubst t sub1.
+Proof.
+  unfold csubst; introv disj.
+  rw <- @csub2sub_app.
+  apply simple_lsubst_app2.
+  - introv i j k.
+    assert (cl_sub (csub2sub sub1)) as cl by eauto 3 with slow.
+    apply in_sub_eta in i; repnd.
+    pose proof (flat_map_free_vars_range_cl_sub (csub2sub sub1) cl) as h.
+    assert (LIn t0 (flat_map free_vars (range (csub2sub sub1)))) as it.
+    { rw lin_flat_map; eexists; dands; eauto. }
+    rw h in it; simpl in it; tcsp.
+  - introv i.
+    assert (prog_sub (csub2sub sub2)) as prog by eauto 3 with slow.
+    rw <- @prog_sub_eq in prog; apply prog.
+    apply in_sub_eta in i; tcsp.
+  - introv i j k.
+    allrw @dom_csub_eq.
+    pose proof (disj v) as xx.
+    rw in_remove_nvars in xx.
+    autodimp xx hyp; tcsp.
+Qed.
+
+Lemma lsubstc_app_weak_r {o} :
+  forall (t : @NTerm o) w x u s1 s2 c,
+    disjoint (remove_nvars [x] (free_vars t)) (dom_csub s2)
+    -> {c' : cover_vars t ((x,u) :: s1)
+        & lsubstc
+            t
+            w
+            ((x,u) :: s1 ++ s2)
+            c
+          = lsubstc t w ((x,u) :: s1) c'}.
+Proof.
+  introv disj.
+
+  assert (cover_vars t ((x,u) :: s1)) as cov.
+  {
+    allrw @cover_vars_eq.
+    allrw subvars_eq.
+    introv i; applydup c in i; allsimpl; clear c.
+    allrw @dom_csub_app.
+    allrw in_app_iff.
+    repndors; tcsp.
+    apply disjoint_sym in disj.
+    apply disj in i0.
+    rw in_remove_nvars in i0; simpl in i0.
+    destruct (deq_nvar x x0); auto.
+    destruct i0; tcsp.
+  }
+
+  exists cov.
+
+  apply lsubstc_eq_if_csubst.
+  rewrite @app_comm_cons.
+  apply subset_free_vars_csub_app3; simpl.
+  introv i.
+  apply disj.
+  allrw in_remove_nvars; repnd; dands; auto.
+  allsimpl.
+  intro j; destruct i; tcsp.
+Qed.
+
+Lemma lsubstc_snoc_weak_r {o} :
+  forall (t : @NTerm o) w x u s y v c,
+    (x <> y -> !LIn y (free_vars t))
+    -> {c' : cover_vars t ((x,u) :: s)
+        & lsubstc
+            t
+            w
+            ((x,u) :: snoc s (y,v))
+            c
+          = lsubstc t w ((x,u) :: s) c'}.
+Proof.
+  introv disj.
+
+  assert (cover_vars t ((x,u) :: s)) as cov.
+  {
+    allrw @cover_vars_eq.
+    allrw subvars_eq.
+    introv i; applydup c in i; allsimpl; clear c.
+    allrw @dom_csub_snoc; allsimpl.
+    allrw in_snoc.
+    repndors; subst; tcsp.
+    destruct (deq_nvar x y); tcsp.
+  }
+
+  exists cov.
+
+  apply lsubstc_eq_if_csubst.
+  rewrite snoc_as_append.
+  rewrite @app_comm_cons.
+  apply subset_free_vars_csub_app3; simpl.
+  introv i j; allsimpl; repndors; subst; tcsp.
+  allrw in_remove_nvars; repnd; allsimpl.
+  allrw not_over_or; repnd; tcsp.
+Qed.
+
+Ltac lsubstc_weak :=
+  match goal with
+  | [ |- context[lsubstc ?t ?w ((?x,?u) :: ?s1 ++ ?s2) ?c] ] =>
+    let disj := fresh "disj" in
+    let h    := fresh "h" in
+    let cov  := fresh "cov" in
+    assert (disjoint (remove_nvars [x] (free_vars t)) (dom_csub s2)) as disj;
+      [ auto
+      | pose proof (lsubstc_app_weak_r t w x u s1 s2 c disj) as h;
+        destruct h as [ cov h ];
+        rewrite h; clear h
+      ]
+
+  | [ |- context[lsubstc ?t ?w ((?x,?u) :: snoc ?s (?y,?v)) ?c] ] =>
+    let disj := fresh "disj" in
+    let h    := fresh "h" in
+    let cov  := fresh "cov" in
+    assert (x <> y -> !LIn y (free_vars t)) as disj;
+      [ auto
+      | pose proof (lsubstc_snoc_weak_r t w x u s y v c disj) as h;
+        destruct h as [ cov h ];
+        rewrite h; clear h
+      ]
+  end.
+
+(* !!MOVE *)
+Lemma isprog_vars_equality {p} :
+  forall (a b c : @NTerm p) vs,
+    isprog_vars vs (mk_equality a b c)
+                <=> (isprog_vars vs a # isprog_vars vs b # isprog_vars vs c).
+Proof.
+  introv.
+  repeat (rw @isprog_vars_eq; simpl).
+  autorewrite with slow.
+  allrw subvars_app_l.
+  allrw <- @wf_term_eq.
+  allrw <- @wf_equality_iff; split; sp.
+Qed.
+
+(* !!MOVE *)
+Lemma isprog_vars_member {p} :
+  forall (a b : @NTerm p) vs,
+    isprog_vars vs (mk_member a b)
+                <=> (isprog_vars vs a # isprog_vars vs b).
+Proof.
+  introv.
+  repeat (rw @isprog_vars_eq; simpl).
+  autorewrite with slow.
+  allrw subvars_app_l.
+  allrw <- @wf_term_eq.
+  allrw <- @wf_equality_iff; split; sp.
+Qed.
+
+(* !!MOVE *)
+Lemma isprog_vars_iff_covered {o} :
+  forall (t : @NTerm o) (vs : list NVar),
+    isprog_vars vs t <=> (covered t vs # wf_term t).
+Proof.
+  tcsp.
+Qed.
+
+(* !!MOVE *)
+Lemma isprog_vars_lsubst2 {o} :
+  forall (t : @NTerm o) vs sub,
+    wf_term t
+    -> (forall v u, LIn (v, u) sub -> isprog_vars vs u)
+    -> isprog_vars (vs ++ dom_sub sub) t
+    -> isprog_vars vs (lsubst t sub).
+Proof.
+  introv w k1 k2.
+  allrw @isprog_vars_eq; repnd.
+  dands.
+
+  {
+    eapply subvars_eqvars;[|apply eqvars_sym; apply eqvars_free_vars_disjoint].
+    rw subvars_app_l; dands.
+
+    - rw subvars_remove_nvars; auto.
+
+    - eapply subvars_trans;[apply sub_free_vars_sub_keep_first_subvars|].
+      rw subvars_eq; introv i.
+      apply in_sub_free_vars in i; exrepnd.
+      apply k1 in i0.
+      apply isprog_vars_eq in i0; repnd.
+      rw subvars_eq in i2; apply i2 in i1; auto.
+  }
+
+  { apply nt_wf_lsubst_iff; dands; auto.
+    introv i j.
+    apply sub_find_some in j.
+    apply k1 in j; eauto 3 with slow.
+  }
+Qed.
+
+(* !!MOVE *)
+Lemma isprog_vars_comm {o} :
+  forall (t : @NTerm o) vs1 vs2,
+    isprog_vars (vs1 ++ vs2) t
+    -> isprog_vars (vs2 ++ vs1) t.
+Proof.
+  introv isp.
+  allrw @isprog_vars_eq; repnd; dands; auto.
+  apply subvars_comm_r; auto.
+Qed.
+
+(* !!MOVE *)
+Lemma isprog_vars_subst2 {o} :
+  forall (t : @NTerm o) v u vs,
+    wf_term t
+    -> isprog_vars vs u
+    -> isprog_vars (v :: vs) t
+    -> isprog_vars vs (subst t v u).
+Proof.
+  introv w k1 k2.
+  apply isprog_vars_lsubst2; simpl; auto.
+
+  - introv i; repndors; cpx.
+
+  - apply isprog_vars_comm; simpl; auto.
+Qed.
+
+Hint Rewrite @vars_hyps_substitute_hyps : slow.
+
+
+(* [23] ============ LAMBDA FORMATION ============ *)
+
+(**
+
+ The following rule is called the lambda formation rules.  It says
+ that to prove that a function type is true, it is enough to prove
+ that given a element [z] in its domain [A], we can prove that its
+ codomain [B[x\z]] is true.  We also have to prove that its domain [A}
+ is a well-formed type.
+<<
+   H |- x:A -> B ext \z.b
+
+     By lambdaFormation lvl(i) z ()
+
+     H , z : A |- B[x\z] ext b
+     H , z : A |- B[x\z] in Type(i)
+     H |- A in Type(i)
+>>
+
+ *)
+
+Definition rule_lambda_formation {o}
+           (A B b e1 e2 : NTerm)
+           (x z  : NVar)
+           (i    : nat)
+           (H    : @barehypotheses o) :=
+  mk_rule
+    (mk_baresequent H (mk_concl (mk_function A x B) (mk_lam z b)))
+    [ mk_baresequent (snoc H (mk_hyp z A))
+                     (mk_concl (subst B x (mk_var z)) b),
+      mk_baresequent (snoc H (mk_hyp z A))
+                     (mk_concl_mem_ext (subst B x (mk_var z)) (mk_uni i) e1),
+      mk_baresequent H (mk_concl_mem_ext A (mk_uni i) e2) ]
+    [sarg_var z].
+
+Lemma rule_lambda_formation_true {o} :
+  forall lib (A B b e1 e2 : NTerm)
+         (x z : NVar)
+         (i   : nat)
+         (H   : @barehypotheses o)
+         (bc1 : !LIn z (bound_vars B)),
+    ext_rule_true lib (rule_lambda_formation A B b e1 e2 x z i H).
+Proof.
+  intros.
+  unfold rule_lambda_formation, ext_rule_true, closed_type_baresequent, closed_extract_baresequent; simpl.
+  intros.
+
+  (* We prove the well-formedness of things *)
+  destseq; allsimpl.
+  dLin_hyp; exrepnd.
+  rename Hyp0 into hyp1.
+  rename Hyp1 into hyp2.
+  rename Hyp2 into hyp3.
+  destseq; allsimpl; proof_irr; GC.
+
+  allunfold @closed_type; allunfold @closed_extract; allsimpl.
+  duplicate wfct as wfi.
+  rw <- @wf_function_iff in wfct.
+  destruct wfct as [ wa wb ].
+  duplicate ce0 as ce.
+  allrw @nh_vars_hyps_snoc; allsimpl.
+
+  assert (covered (mk_lam z b) (nh_vars_hyps H)) as cv.
+  { clear hyp1 hyp2 hyp3.
+    allunfold @covered; allsimpl; allrw app_nil_r.
+    autorewrite with core list in *.
+    allrw @nh_vars_hyps_snoc.
+    allrw subvars_remove_nvars.
+    allrw <- snoc_as_append; sp. }
+
+  exists cv; GC.
+
+  (* We prove some simple facts on our sequents *)
+  assert ((z <> x -> !LIn z (free_vars B))
+          # !LIn z (free_vars A)
+          # !LIn z (vars_hyps H)) as vhyps.
+  {
+    clear hyp1 hyp2 hyp3.
+    dwfseq.
+    sp;
+      try (complete (generalize (cg z); sp;
+                     allrw in_remove_nvars; allsimpl;
+                     autodimp X0 h; sp));
+      try (complete (apply_in_hyp p;
+                     generalize (subvars_hs_vars_hyps H); intro sv;
+                     rw subvars_prop in sv;
+                     apply sv in p; sp)).
+  }
+
+  destruct vhyps as [ nzB vhyps ].
+  destruct vhyps as [ nzA nzH ].
+  (* done with proving these simple facts *)
+
+  (* we now start proving the sequent *)
+  ext_seq_true.
+
+  lsubst_tac.
+
+  dands; apply equality_in_function; dands.
+
+  {
+    ext_seq_true in hyp3.
+    pose proof (hyp3 s1 s2 sim) as q; exrepnd.
+    lsubst_tac.
+    apply member_if_inhabited in q0; eauto 3 with slow.
+  }
+
+  {
+    introv equa.
+    ext_seq_true in hyp2.
+    pose proof (hyp2 (snoc s1 (z,a)) (snoc s2 (z,a'))) as q; exrepnd.
+    autodimp q hyp.
+
+    { sim_snoc; dands; auto. }
+
+    exrepnd.
+    lsubst_tac.
+    apply equality_in_member in q0.
+    apply equality_in_member in q1.
+    exrepnd.
+    spcast; computes_to_eqval.
+
+    assert (cequivc lib (mkc_prefl x1 z1) (mkc_prefl x0 z0)) as ceq.
+    { eapply cequivc_trans;
+        [apply cequivc_sym;apply computes_to_valc_implies_cequivc;eauto|].
+      apply computes_to_valc_implies_cequivc; auto. }
+
+Definition type_family2 {p} lib TyCon (ts : cts(p)) (T : @CTerm p) eqa eqb : [U]:=
+  {A : CTerm
+  , {v : NVar
+  , {B : CVTerm [v]
+  , T ===>(lib) (TyCon A v B)
+  # ts A eqa
+  # (forall a a' (e : eqa a a'), ts (B[[v\\a]]) (eqb a a' e))
+  # per_fam_equiv eqb
+  # (forall T' A' v B' eq' eqa' eqb',
+        T' ===>(lib) (TyCon A' v' B')
+        -> ts A' eqa'
+        -> ts T' eq'
+        -> eqa' <=2=> eqa
+        -> (eq' <=2=> (per_func_eq eqa eqb))
+        -> (forall a a' (e : eqa' a a'), ts (B'[[v\\a]]) (eqb' a a' e))
+        -> (forall a a' (e : eqa a a') (e' : eqa' a a'), (eqb a a' e) <=2=> (eqb' a a' e'))
+    }}}.
+
+SearchAbout similarity.
+    SearchAbout cequivc mkc_pair.
+
+XXXXXXXX
+
+    assert (@wf_term o (mk_var z)) as wfz.
+    { eauto 3 with slow. }
+
+    assert (cover_vars (mk_var z) (snoc s1 (z, a))) as cov1z.
+    { apply cover_vars_var; rw @dom_csub_snoc; simpl; rw in_snoc; tcsp. }
+
+    assert (cover_vars (mk_var z) (snoc s1 (z, a'))) as cov1z'.
+    { apply cover_vars_var; rw @dom_csub_snoc; simpl; rw in_snoc; tcsp. }
+
+    assert (cover_vars (mk_var z) (snoc s2 (z, a))) as cov2z.
+    { apply cover_vars_var; rw @dom_csub_snoc; simpl; rw in_snoc; tcsp. }
+
+    assert (cover_vars (mk_var z) (snoc s2 (z, a'))) as cov2z'.
+    { apply cover_vars_var; rw @dom_csub_snoc; simpl; rw in_snoc; tcsp. }
+
+    repeat (lsubstc_subst_aeq2;[]).
+    repeat (substc_lsubstc_vars3;[]).
+    repeat (lsubstc_weak;[]).
+    proof_irr; auto.
+  }
+
+XXXXXXXX
+
+  (* We prove our first subgoal *)
+  assert (forall s2 pC2,
+            similarity lib s1 s2 H
+            -> tequality
+                 lib
+                 (lsubstc (mk_function A x B) wfi s1 pC1)
+                 (lsubstc (mk_function A x B) wfi s2 pC2)) as tfb.
+  {
+    clear s2 pC2 pt2 sim.
+    intros s2 pC2 sim.
+    lift_lsubst.
+    apply implies_tequality_function.
+
+    - vr_seq_true in hyp2.
+      pose proof (hyp2 s1 s2) as hyp2.
+      repeat (autodimp hyp2 h); exrepnd.
+      lsubst_tac.
+      allrw @fold_mkc_member.
+      apply equality_in_member in hyp2; exrepnd; eauto 3 with slow.
+      apply tequality_mkc_member_implies_equality in hyp0; eauto 3 with slow.
+
+    - (* we use our 1st hypothesis to prove that B is a type family *)
+      introv equ.
+      vr_seq_true in hyp1.
+      generalize (hyp1 (snoc s1 (z, a)) (snoc s2 (z, a'))); clear hyp1; intro hyp1.
+      autodimp hyp1 h.
+
+      {
+        (* To use our 1st hyp, we first have to prove that the hypotheses are functional *)
+        intros s3 sim3.
+        inversion sim3; cpx; allsimpl; cpx; clear_irr.
+        assert (cover_vars A s4) as c4
+            by (apply similarity_cover_vars with (t := A) in sim0; auto).
+        (* we use our hyp (coming from proving that our sequent is true) that says that H is functional *)
+        rw @eq_hyps_snoc; simpl.
+
+        exists s1 s4 a t2 wa c1 c4; sp.
+        (* now to prove that functionality statement on A, we use our 2nd hyp *)
+        vr_seq_true in hyp2.
+        generalize (hyp2 s1 s4); clear hyp2; intro hyp2.
+        autodimp hyp2 hyp.
+        autodimp hyp2 hyp; exrepd.
+        lsubst_tac.
+        allrw @fold_mkc_member.
+        apply equality_in_member in e1; exrepnd; eauto 3 with slow.
+        eapply tequality_in_uni_implies_tequality in t; eauto 3 with slow.
+        apply equality_refl in e4.
+        apply t in e4; eauto 3 with slow.
+      }
+      (* and we're done proving that the hypotheses are functional *)
+
+      (* now we can keep using our 1st hypothesis *)
+      autodimp hyp1 hyp.
+
+      {
+        (* For that we have to prove that the two terms we picked to be equal in A are actually equal in A *)
+        sim_snoc2; dands; auto; proof_irr; auto.
+      }
+      (* easy enough *)
+
+      (* and again, we keep on using our 1st hypothesis *)
+      exrepd. (* we prove that from t *)
+
+      assert (lsubstc (subst B x (mk_var z)) wfct1 (snoc s1 (z, a)) pC0
+              = substc a x (lsubstc_vars B wb (csub_filter s1 [x]) [x] c2)) as eq1
+          by (apply lsubstc_subst_snoc_eq; try (complete sp);
+              allapply @similarity_dom; exrepd; allrw; sp).
+
+      rewrite eq1 in t.
+
+      assert (lsubstc (subst B x (mk_var z)) wfct1 (snoc s2 (z, a')) pC3
+              = substc a' x (lsubstc_vars B wb (csub_filter s2 [x]) [x] c3)) as eq2
+          by (apply lsubstc_subst_snoc_eq; try (complete sp);
+              allapply @similarity_dom; exrepd; allrw; sp).
+
+      rewrite eq2 in t.
+      auto.
+      (* and we're done proving our 1st subgoal (the tequality) *)
+  }
+
+  (* We now prove our second subgoal *)
+  dands; tcsp.
+  lift_lsubst.
+  applydup @similarity_refl in sim.
+  rw @equality_in_function.
+
+  dands.
+  (* We have to prove 3 goals *)
+
+  {
+    (* 1) we have to prove that A is a type *)
+    generalize (tfb s1 pC1 sim0); sp.
+    lsubst_tac.
+    allrw @tequality_function; sp.
+  }
+
+  {
+    (* 2) we have to prove that B is a type family *)
+    generalize (tfb s1 pC1 sim0); sp.
+    lsubst_tac.
+    allrw @tequality_function; sp.
+  }
+
+  {
+    (* 3) we have to prove that b is a member B *)
+    vr_seq_true in hyp1.
+    introv eqa.
+    generalize (hyp1 (snoc s1 (z, a)) (snoc s2 (z, a'))); clear hyp1; intro hyp1.
+    autodimp hyp1 hyp.
+
+    {
+      (* first we have to prove that the hypotheses are functional *)
+      intros s3 sim3.
+      inversion sim3; cpx; allsimpl; cpx; clear_irr.
+      assert (cover_vars A s4) as c4
+          by (apply similarity_cover_vars with (t := A) in sim1; auto).
+      (* we use our hyp (coming from proving that our sequent is true) that says that H is functional *)
+      allapplydup eqh.
+      rw @eq_hyps_snoc; simpl.
+      exists s1 s4 a t2 wa c1 c4; sp.
+      (* now to prove that functionality statement on A, we use our 2nd hyp (from tfb) *)
+
+      vr_seq_true in hyp2.
+      pose proof (hyp2 s1 s4) as hyp2.
+      repeat (autodimp hyp2 hyp); exrepnd.
+      lsubst_tac.
+      allrw @fold_mkc_member.
+      apply equality_in_member in hyp1; exrepnd; eauto 3 with slow.
+      apply tequality_mkc_member_implies_equality in hyp0; eauto 3 with slow.
+      (* and we're done proving that the hypotheses are functional *)
+    }
+
+    (* now we can keep using our 1st hypothesis *)
+    autodimp hyp1 hyp.
+
+    {
+      (* For that we have to prove that the two terms we picked to be equal in A are actually equal in A *)
+      rw @similarity_snoc; simpl.
+      exists s1 s2 a a' wa c1; sp.
+      (* easy enough *)
+    }
+
+    (* and again, we keep on using our 1st hypothesis *)
+    exrepd. (* we prove that from e *)
+    clear t; clear_irr.
+
+    assert (lsubstc (subst B x (mk_var z)) wfct1 (snoc s1 (z, a)) pC0
+            = substc a x (lsubstc_vars B wb (csub_filter s1 [x]) [x] c2)) as eq1.
+    {
+      rewrite substc_eq_lsubstc; simpl.
+      apply lsubstc_eq_if_csubst.
+      rewrite csubst_app.
+      unfold subst, csubst.
+      try (rw lsubstn_lsubst; try (complete (simpl; rw disjoint_singleton_r; sp))).
+      rewrite simple_lsubst_lsubst;
+        try (complete (sp; allapply @in_csub2sub; sp));
+        try (complete (simpl; sp; cpx; simpl; apply disjoint_singleton_l; auto)).
+      rewrite lsubst_sub_singleton.
+      rewrite fold_csubst.
+      rewrite csubst_snoc_var;
+        try (complete (allapply @similarity_dom; exrepd; allrw; sp)).
+      rewrite <- csub2sub_app; simpl.
+      rewrite <- snoc_as_append.
+      rewrite <- lsubst_swap;
+        try (complete (sp; allapply @in_csub2sub; sp));
+        try (complete (rewrite @dom_csub_eq; rewrite @dom_csub_csub_filter; rw in_remove_nvars; simpl; sp)).
+      repeat (rewrite <- @csub2sub_cons).
+      repeat (rewrite @fold_csubst).
+      destruct (eq_var_dec z x); subst.
+      (* if they're equal it's easy *)
+      rewrite csubst_cons_trim.
+      rewrite csub_filter_snoc1; sp.
+      (* if they're not: *)
+      rewrite <- csubst_csub_filter with (l := [z]);
+        try (rw disjoint_singleton_r; sp).
+      assert (x <> z) as d by auto; simpl.
+      apply memvar_singleton_diff_r in d; rewrite d.
+      rewrite csub_filter_snoc1; sp.
+      rewrite csubst_cons_trim.
+      rewrite <- csub_filter_app_r; simpl.
+      symmetry.
+      rewrite <- csubst_csub_filter with (l := [z]); simpl;
+        try (rw disjoint_singleton_r; sp).
+      rewrite d.
+      rewrite csub_filter_swap.
+      rewrite <- csub_filter_app_r; sp.
+    }
+
+    rewrite eq1 in e0; clear eq1.
+
+    lsubst_tac; sp.
+
+    assert (cequivc lib
+                    (lsubstc b wfce1 (snoc s1 (z, a)) pt0)
+                    (mkc_apply
+                       (mkc_lam z (lsubstc_vars b wfce1 (csub_filter s1 [z]) [z] c0))
+                       a)) as ceq1.
+    {
+      apply cequivc_sym.
+      revert c0; rw @csub_filter_trivial; introv;
+        try (complete (simpl; sp; subst; allapply @similarity_dom; repnd; allrw sim1; sp)).
+      destruct_cterms; unfold cequivc; simpl; unfold csubst; simpl.
+      allrw @csub2sub_snoc; simpl.
+      generalize (cequiv_beta lib z (lsubst b (csub2sub s1)) x1); introv ceq1.
+      autodimp ceq1 hyp.
+      apply csubst.isprog_vars_lsubst.
+      introv k; allrw @in_range_iff; exrepnd; allapply @in_csub2sub; sp.
+      simpl.
+      rw @isprog_vars_eq; sp.
+      allunfold @covered.
+      rw @dom_csub_eq.
+      allapply @similarity_dom; repnd; allrw.
+      apply subvars_trans with (vs2 := snoc (nh_vars_hyps H) z); sp.
+      rw subvars_prop; introv j; allsimpl; allrw in_snoc; sp.
+      generalize (subset_hs_vars_hyps H); intro k.
+      right; apply k; sp.
+      rw @nt_wf_eq; sp.
+      autodimp ceq1 hyp.
+      allrw @isprogram_eq; sp.
+      rw @simple_lsubst_snoc in ceq1; sp.
+      rw @isprogram_eq; sp.
+      allapply @in_csub2sub; sp.
+    }
+
+    assert (cequivc lib
+                    (lsubstc b wfce1 (snoc s2 (z, a')) pt3)
+                    (mkc_apply
+                       (mkc_lam z (lsubstc_vars b wfce1 (csub_filter s2 [z]) [z] c3))
+                       a'))
+      as ceq2.
+    {
+      apply cequivc_sym.
+      revert c3; rw @csub_filter_trivial; introv;
+        try (complete (simpl; sp; subst; allapply @similarity_dom; repnd; allrw sim; sp)).
+      destruct_cterms; unfold cequivc; simpl; unfold csubst; simpl.
+      allrw @csub2sub_snoc; simpl.
+      generalize (cequiv_beta lib z (lsubst b (csub2sub s2)) x0); introv ceq2.
+      autodimp ceq2 hyp.
+      apply csubst.isprog_vars_lsubst.
+      introv k; allrw @in_range_iff; exrepnd; allapply @in_csub2sub; sp.
+      simpl.
+      rw @isprog_vars_eq; sp.
+      allunfold @covered.
+      rw @dom_csub_eq.
+      allapply @similarity_dom; repnd; allrw.
+      apply subvars_trans with (vs2 := snoc (nh_vars_hyps H) z); sp.
+      rw subvars_prop; introv j; allsimpl; allrw in_snoc; sp.
+      generalize (subset_hs_vars_hyps H); intro k.
+      right; apply k; sp.
+      rw @nt_wf_eq; sp.
+      autodimp ceq2 hyp.
+      allrw @isprogram_eq; sp.
+      rw @simple_lsubst_snoc in ceq2; sp.
+      rw @isprogram_eq; sp.
+      allapply @in_csub2sub; sp.
+    }
+
+    apply @equality_respects_cequivc_left with (t1 := lsubstc b wfce1 (snoc s1 (z, a)) pt0); sp.
+    apply @equality_respects_cequivc_right with (t2 := lsubstc b wfce1 (snoc s2 (z, a')) pt3); sp.
+  }
+Qed.
+
+(* begin hide *)
+
+Lemma rule_lambda_formation_true_ex {p} :
+  forall lib i z A B b e x H (bc1 : !LIn z (bound_vars B)),
+    @rule_true_if p lib (rule_lambda_formation A B b e x z i H).
+Proof.
+  intros.
+  generalize (rule_lambda_formation_true lib A B b e x z i H bc1); intro rt.
+  rw <- @rule_true_eq_ex in rt.
+  unfold rule_true_ex in rt; sp.
+Qed.
+
+(* [24] ============ FUNCTION EQUALITY ============ *)
+
+(**
+
+  The following rule is called the function equality rule.  It says
+  that to prove that a function type is well-formed, we have to prove
+  that its domain is well-formed and that its co-domain is functional
+  over its domain.
+<<
+   H |- x1:a1 -> b1 = x2:a2 -> b2 in Type(i)
+
+     By functionEquality y ()
+
+     H |- a1 = a2 in Type(i)
+     H y : a1 |- subst b1 x1 y = subst b2 x2 y in Type(i)
+>>
+ *)
+
+Definition rule_function_equality {p}
+           (a1 a2 b1 b2 e1 e2 : NTerm)
+           (x1 x2 y : NVar)
+           (i   : nat)
+           (H   : @barehypotheses p) :=
+  mk_rule
+    (mk_baresequent
+       H
+       (mk_concl_eq (mk_function a1 x1 b1)
+                    (mk_function a2 x2 b2)
+                    (mk_uni i)))
+    [ mk_baresequent H (mk_concl_eq_ext a1 a2 (mk_uni i) e1),
+      mk_baresequent
+        (snoc H (mk_hyp y a1))
+        (mk_concl_eq_ext (subst b1 x1 (mk_var y))
+                         (subst b2 x2 (mk_var y))
+                         (mk_uni i)
+                         e2)
+    ]
+    [ sarg_var y , sarg_term (mk_function a1 x1 b1) ].
+
+Lemma rule_function_equality_true3 {o} :
+  forall lib (a1 a2 b1 b2 e1 e2 : NTerm)
+         (x1 x2 y : NVar)
+         (i   : nat)
+         (H   : @barehypotheses o),
+    rule_true3 lib (rule_function_equality
+                     a1 a2 b1 b2 e1 e2
+                     x1 x2 y
+                     i
+                     H).
+Proof.
+  intros.
+  apply (rule_tyfam_equality_true3 _ _ mkc_function).
+
+  - introv; simpl; allrw remove_nvars_nil_l; allrw app_nil_r; auto.
+
+  - introv; apply lsubstc_mk_function_ex.
+
+  - apply implies_tequalityi_function; auto.
+Qed.
+
+Lemma rule_function_equality_true {o} :
+  forall lib (a1 a2 b1 b2 e1 e2 : NTerm)
+         (x1 x2 y : NVar)
+         (i   : nat)
+         (H   : @barehypotheses o),
+    rule_true lib (rule_function_equality
+                     a1 a2 b1 b2 e1 e2
+                     x1 x2 y
+                     i
+                     H).
+Proof.
+  introv.
+  apply rule_true3_implies_rule_true.
+  apply rule_function_equality_true3.
+Qed.
+
+(* begin hide *)
+
+
+Lemma rule_function_equality_true_ex {o} :
+  forall lib y i a1 a2 b1 b2 e1 e2 x1 x2 H,
+    @rule_true_if o lib (rule_function_equality a1 a2 b1 b2 e1 e2 x1 x2 y i H).
+Proof.
+  intros.
+  generalize (rule_function_equality_true lib a1 a2 b1 b2 e1 e2 x1 x2 y i H); intro rt.
+  rw <- @rule_true_eq_ex in rt.
+  unfold rule_true_ex in rt; sp.
+Qed.
+
+
+
+(* [27] ============ APPLY REDUCE ============ *)
+
+(**
+
+  The following rule called the ``apply reduce'' rule is the
+  computation rule for applications.
+<<
+   H |- (\x.t)s = u in T
+
+     By applyReduce ()
+
+     H |- t[x\s] = u in T
+>>
+ *)
+
+Definition rule_apply_reduce {o}
+           (T t s u e : NTerm)
+           (x : NVar)
+           (H : @barehypotheses o) :=
+  mk_rule
+    (mk_baresequent
+       H
+       (mk_concl_eq_ext (mk_apply (mk_lam x t) s) u T e))
+    [ mk_baresequent
+        H
+        (mk_concl_eq_ext (subst t x s) u T e)
+    ]
+    [].
+
+Lemma rule_apply_reduce_true {o} :
+  forall lib (T t s u e : NTerm)
+         (x   : NVar)
+         (H   : @barehypotheses o)
+         (bc1 : disjoint (free_vars s) (bound_vars t)),
+    rule_true lib (rule_apply_reduce T t s u e x H).
+Proof.
+  intros.
+  unfold rule_apply_reduce, rule_true, closed_type_baresequent, closed_extract_baresequent; simpl.
+  intros.
+
+  (* We prove the well-formedness of things *)
+  destseq; allsimpl.
+  dLin_hyp; exrepnd.
+  rename Hyp0 into hyp1.
+  destseq; allsimpl; proof_irr; GC.
+
+  allunfold @closed_type; allunfold @closed_extract; allsimpl.
+  duplicate wfct as wfi.
+  rw <- @wf_equality_iff in wfct.
+  destruct wfct as [ wa wfct ].
+  destruct wfct as [ wu wT ].
+  rw <- @wf_apply_iff in wa.
+  destruct wa as [ wt ws ].
+  rw <- @wf_lam_iff in wt.
+
+  match goal with
+  | [ |- context[covered ?a ?b] ] => assert (covered a b) as cov by auto
+  end.
+  exists cov.
+
+  (* We prove some simple facts on our sequents *)
+  (* xxx *)
+  (* done with proving these simple facts *)
+
+  (* we now start proving the sequent *)
+  vr_seq_true.
+  vr_seq_true in hyp1.
+  generalize (hyp1 s1 s2 eqh sim); clear hyp1; intro hyp1; exrepnd.
+
+  lsubst_tac.
+  dands.
+
+  {
+    eapply tequality_respects_cequivc_left;
+      [apply cequivc_sym;apply cequivc_decomp_equality;dands;
+       [apply cequivc_beta|apply cequivc_refl|apply cequivc_refl]
+      |].
+    eapply tequality_respects_cequivc_right;
+      [apply cequivc_sym;apply cequivc_decomp_equality;dands;
+       [apply cequivc_beta|apply cequivc_refl|apply cequivc_refl]
+      |].
+
+    repeat (substc_lsubstc_vars3;[]).
+    clear_irr; auto.
+  }
+
+  {
+    eapply cequivc_preserving_equality;
+      [|apply cequivc_sym;apply cequivc_decomp_equality;dands;
+        [apply cequivc_beta|apply cequivc_refl|apply cequivc_refl]
+      ].
+
+    repeat (substc_lsubstc_vars3;[]).
+    clear_irr; auto.
+  }
+Qed.
+
+
+Definition singleton_type {o} v (a A : @CTerm o) : CTerm :=
+  mkc_set A v (mkcv_equality [v] (mkc_var v) (mk_cv [v] a) (mk_cv [v] A)).
+
+Lemma ext_eq_function_implies_ext_eq_singleton {o} :
+  forall lib (A : @CTerm o) v1 v2 B1 B2 a v,
+    member lib a A
+    -> ext_eq lib (mkc_function A v1 B1) (mkc_function A v2 B2)
+    -> ext_eq lib (mkc_function (singleton_type v a A) v1 B1) (mkc_function (singleton_type v a A) v2 B2).
+Proof.
+  introv mem ext.
+
+  introv; split; intro h.
+
+  (* This is not true: Take
+       T1 = v:Int->B1[v], where B1[v] = if v=0 then Void else Unit
+       T2 = v:Int->B2[v], where B2[v] = if v=1 then Void else Unit
+     These two types are empty because of the use of Void.
+     We don't have {0}->B1[0] = {0}->B2[0] because this is equivalent to
+     {0}->Void = {0}->Unit, and these two types are not extensionally equal.
+
+     Here, the pi type is empty though, while in our proof, it isn't.
+     Can we find a counter-example where the type is not empty?
+   *)
+Abort.
+
+
+
+(**
+
+Same as functionElimination with one additional well-formedness subgoal for
+the B family.
+
+<<
+   H, f : x:A->B[x], J |- C ext e[z\(f a)]
+
+     By functionElimination s z
+
+     H, f : x:A->B[x], J |- a in A
+     H, f : x:A->B[x], J, z : (f a) in B[a] |- C ext e
+     H, f : x:A->B[x], J |- B[a] in U(i)
+>>
+
+ *)
+
+Definition rule_function_elimination_wf_concl {o}
+           (A : @NTerm o) B C a e f x z H J :=
+  mk_baresequent
+    (snoc H (mk_hyp f (mk_function A x B)) ++ J)
+    (mk_concl C (subst e z (mk_prefl (mk_apply (mk_var f) a) (mk_apply (mk_var f) a)))).
+
+Definition rule_function_elimination_wf_hyp1 {o}
+           (A : @NTerm o) B a e f x H J :=
+  mk_baresequent
+    (snoc H (mk_hyp f (mk_function A x B)) ++ J)
+    (mk_concl (mk_member a A) e).
+
+Definition rule_function_elimination_wf_hyp2 {o}
+           (A : @NTerm o) B C a e f x z H J :=
+  mk_baresequent
+    (snoc (snoc H (mk_hyp f (mk_function A x B)) ++ J)
+          (mk_hyp z (mk_member (mk_apply (mk_var f) a)
+                               (subst B x a))))
+    (mk_concl C e).
+
+Definition rule_function_elimination_wf_hyp3 {o}
+           (A : @NTerm o) B a e f x H J i :=
+  mk_baresequent
+    (snoc H (mk_hyp f (mk_function A x B)) ++ J)
+    (mk_concl_mem_ext (subst B x a) (mk_uni i) e).
+
+Definition rule_function_elimination_wf {p}
+           (A B C a e1 e2 e3 : NTerm)
+           (f x z : NVar)
+           (H J : @barehypotheses p)
+           (i : nat) :=
+  mk_rule
+    (rule_function_elimination_wf_concl A B C a e2 f x z H J)
+    [
+      rule_function_elimination_wf_hyp1 A B a e1 f x H J,
+      rule_function_elimination_wf_hyp2 A B C a e2 f x z H J,
+      rule_function_elimination_wf_hyp3 A B a e3 f x H J i
+    ]
+    [ sarg_term a (*, sarg_var z*)].
+
+Lemma rule_function_elimination_wf_true3 {p} :
+  forall lib (A B C a e1 e2 e3 : NTerm)
+         (f x z : NVar)
+         (H J : @barehypotheses p)
+         (i : nat),
+    rule_true3 lib (rule_function_elimination_wf
+                      A B C a e1 e2 e3
+                      f x z
+                      H J
+                      i).
+Proof.
+  unfold rule_function_elimination_wf, rule_true3, wf_bseq, closed_type_baresequent, closed_extract_baresequent; simpl.
+  intros; repnd.
+
+  pose proof (cargs (sarg_term a)) as ca.
+  simpl in ca; autodimp ca hyp.
+  rw @nh_vars_hyps_app in ca; simpl in ca.
+  rw @nh_vars_hyps_snoc in ca; simpl in ca.
+
+  (* We prove the well-formedness of things *)
+  destseq; allsimpl.
+  dLin_hyp; exrepnd.
+  rename Hyp into hyp1.
+  rename Hyp0 into hyp2.
+  rename Hyp1 into hyp3.
+  destruct hyp1 as [ ws1 hyp1 ].
+  destruct hyp2 as [ ws2 hyp2 ].
+  destruct hyp3 as [ ws3 hyp3 ].
+  destseq; allsimpl; proof_irr; GC.
+
+  assert (wf_csequent (rule_function_elimination_wf_concl A B C a e2 f x z H J)) as wfc.
+  {
+    clear hyp1 hyp2 hyp3.
+    unfold wf_csequent, closed_type, closed_extract, wf_sequent, wf_concl; simpl.
+    prove_seq; eauto 3 with slow.
+    { apply wf_term_subst; eauto 3 with slow.
+      apply wf_prefl; dands;
+        apply wf_apply; eauto 2 with slow. }
+    apply covered_subst; eauto 2 with slow.
+    { eapply covered_subvars;[|eauto].
+      autorewrite with slow; simpl.
+      rw subvars_eq; introv j; simpl.
+      repeat (allrw @in_snoc; allrw @in_app_iff).
+      repndors; tcsp. }
+    { apply covered_prefl_same.
+      apply covered_apply; dands; eauto 3 with slow.
+      apply covered_var; rw in_app_iff; rw in_snoc; tcsp. }
+  }
+  exists wfc.
+  unfold wf_csequent, wf_sequent, wf_concl in wfc; allsimpl; repnd; proof_irr; GC.
+
+  (* We prove some simple facts on our sequents *)
+  assert (disjoint (free_vars A) (vars_hyps J)
+          # disjoint (remove_nvars [x] (free_vars B)) (vars_hyps J)
+          # subvars (free_vars a) (snoc (vars_hyps H) f ++ vars_hyps J)
+          # wf_term a
+          # !LIn z (free_vars C)
+          # !LIn z (vars_hyps H)
+          # !LIn z (vars_hyps J)
+          # (z <> f)
+          # !LIn f (vars_hyps H)
+          # !LIn f (vars_hyps J)
+          # !LIn f (free_vars A)
+          # (x <> f -> !LIn f (free_vars B))) as vhyps.
+  {
+    clear hyp1 hyp2.
+    dwfseq.
+    sp;
+      try (complete (introv j; discover; allunfold @disjoint; discover; auto));
+      try (complete (assert (LIn f (remove_nvars [x] (free_vars B)))
+                      by (rw in_remove_nvars; rw in_single_iff; sp);
+                     discover; auto));
+      try (complete (apply wf_member_iff in wfct1; sp));
+      try (complete (generalize (wfh10 z); rw in_app_iff; rw in_snoc; sp));
+      try (complete (generalize (wfh10 f); rw in_remove_nvars; simpl; intro j;
+                     dest_imp j hyp));
+      try complete (pose proof (wfc1 z) as xx; autodimp xx hyp;
+                    rw in_app_iff in xx; rw in_snoc in xx; repndors; tcsp).
+  }
+
+  destruct vhyps as [ daj  vhyps ].
+  destruct vhyps as [ dbj  vhyps ].
+  destruct vhyps as [ sva  vhyps ].
+  destruct vhyps as [ wa   vhyps ].
+  destruct vhyps as [ nizc vhyps ].
+  destruct vhyps as [ nizh vhyps ].
+  destruct vhyps as [ nizj vhyps ].
+  destruct vhyps as [ nzf  vhyps ].
+  destruct vhyps as [ nifh vhyps ].
+  destruct vhyps as [ nifj vhyps ].
+  destruct vhyps as [ nifa nifb ].
+  (* done with proving these simple facts *)
+
+  vr_seq_true.
+
+  duplicate sim as simapp.
+
+  rw @similarity_app in sim; simpl in sim; exrepnd; subst; cpx.
+  rw @similarity_snoc in sim5; simpl in sim5; exrepnd; subst; cpx.
+  lsubst_tac.
+  rw @equality_in_function in sim2; repnd.
+
+  vr_seq_true in hyp2.
+
+  assert (cover_vars a (snoc s1a0 (f, t1) ++ s1b)) as cova1.
+  {
+    apply cover_vars_eq.
+    rw @dom_csub_app; rw @dom_csub_snoc; simpl.
+    clear hyp1 hyp2 hyp3; revert ct1.
+    unfold covered; simpl; autorewrite with slow.
+    repeat (rw @subvars_app_l).
+    introv h; repnd; clear h; GC.
+    rw @vars_hyps_app in h0; rw @vars_hyps_snoc in h0; simpl in h0.
+    apply similarity_dom in sim6; repnd; allrw.
+    apply similarity_dom in sim1; repnd; allrw.
+    autorewrite with slow; auto.
+  }
+
+  assert (cover_vars a (snoc s2a0 (f, t2) ++ s2b)) as cova2.
+  {
+    apply cover_vars_eq.
+    rw @dom_csub_app; rw @dom_csub_snoc; simpl.
+    clear hyp1 hyp2 hyp3; revert ct1.
+    unfold covered; simpl; autorewrite with slow.
+    repeat (rw @subvars_app_l).
+    introv h; repnd; clear h; GC.
+    rw @vars_hyps_app in h0; rw @vars_hyps_snoc in h0; simpl in h0.
+    apply similarity_dom in sim6; repnd; allrw.
+    apply similarity_dom in sim1; repnd; allrw.
+    autorewrite with slow; auto.
+  }
+
+  generalize (hyp2 (snoc (snoc s1a0 (f, t1) ++ s1b)
+                         (z, mkc_prefl (mkc_apply t1 (lsubstc a wa (snoc s1a0 (f, t1) ++ s1b) cova1))
+                                       (mkc_apply t1 (lsubstc a wa (snoc s1a0 (f, t1) ++ s1b) cova1))))
+                   (snoc (snoc s2a0 (f, t2) ++ s2b)
+                         (z, mkc_prefl (mkc_apply t2 (lsubstc a wa (snoc s2a0 (f, t2) ++ s2b) cova2))
+                                       (mkc_apply t2 (lsubstc a wa (snoc s2a0 (f, t2) ++ s2b) cova2)))));
+    clear hyp2; intros hyp2.
+  repeat (autodimp hyp2 h); exrepnd.
+
+  {
+    (* hyps_functionality *)
+
+    apply hyps_functionality_snoc2; simpl; auto;[].
+    introv equ sim; GC; lsubst_tac.
+
+    apply equality_in_member in equ.
+    exrepnd; computes_to_value_isvalue.
+
+    assert (equality lib (lsubstc a wa (snoc s1a0 (f, t1) ++ s1b) cova1)
+                     (lsubstc a wa s' c4)
+                     (lsubstc A w1 s1a0 c1)) as eqa.
+    {
+      vr_seq_true in hyp1.
+      generalize (hyp1 (snoc s1a0 (f, t1) ++ s1b) s'); clear hyp1; intros hyp1.
+      repeat (autodimp hyp1 h); exrepnd.
+      lsubst_tac.
+      allapply @member_if_inhabited.
+      apply tequality_mkc_member_implies_equality in hyp0; auto.
+    }
+
+    apply implies_tequality_mkc_member_if_equal; auto.
+
+    {
+      vr_seq_true in hyp3.
+      pose proof (hyp3 (snoc s1a0 (f, t1) ++ s1b) s') as q.
+      repeat (autodimp q hyp).
+      exrepnd.
+      lsubst_tac.
+      apply member_if_inhabited in q1.
+      apply tequality_if_tequality_in_uni in q0; auto.
+    }
+
+    rw @similarity_app in sim; simpl in sim; exrepnd; subst; cpx.
+    apply app_split in sim7; repnd; allrw length_snoc;
+      try (complete (allrw; sp)); subst; cpx.
+    rw @similarity_snoc in sim12; simpl in sim12; exrepnd; subst; cpx.
+    lsubst_tac.
+    rw @equality_in_function in sim9; repnd.
+    applydup sim9 in eqa as eqf.
+
+    assert (disjoint (remove_nvars [x] (free_vars B)) (dom_csub s1b0)) as disj1.
+    {
+      apply similarity_dom in sim1; repnd.
+      allrw; autorewrite with slow; auto.
+    }
+
+    assert (disjoint (remove_nvars [x] (free_vars B)) (dom_csub s2b0)) as disj2.
+    {
+      apply similarity_dom in sim8; repnd.
+      allrw; autorewrite with slow; auto.
+    }
+
+    repeat (lsubstc_subst_aeq2;[]).
+    repeat (substc_lsubstc_vars3;[]).
+    repeat (lsubstc_weak;[]).
+    proof_irr; auto.
+  }
+
+
+  {
+    (* similarity *)
+
+    assert (wf_term (mk_member (mk_apply (mk_var f) a) (subst B x a))) as wm.
+    {
+      apply wf_member; sp; try (apply wf_apply; sp).
+      apply subst_preserves_wf_term; sp.
+    }
+
+    assert (cover_vars (mk_member (mk_apply (mk_var f) a) (subst B x a))
+                       (snoc s1a0 (f, t1) ++ s1b)) as cm.
+    {
+      apply cover_vars_member; sp.
+      apply cover_vars_apply; sp.
+      { apply cover_vars_var.
+        rw @dom_csub_app; rw @dom_csub_snoc; rw in_app_iff; rw in_snoc; simpl; sp. }
+      rw @cover_vars_eq; rw @cover_vars_covered; apply covered_subst; sp.
+      rw @dom_csub_app; rw @dom_csub_snoc; simpl.
+      rw cons_app; apply covered_app_weak_l.
+      clear sim2 sim5; unfold cover_vars_upto in c2; unfold covered.
+      prove_subvars c2; allsimpl; sp.
+      rw @dom_csub_csub_filter in l; rw in_remove_nvars in l; rw in_single_iff in l.
+      rw in_snoc; sp.
+    }
+
+    sim_snoc.
+    dands; auto.
+    lsubst_tac.
+    apply equality_in_member.
+
+    assert (disjoint (remove_nvars [x] (free_vars B)) (dom_csub s1b)) as disj0.
+    {
+      apply similarity_dom in sim1; repnd.
+      allrw; autorewrite with slow; auto.
+    }
+
+    vr_seq_true in hyp1.
+    generalize (hyp1 (snoc s1a0 (f, t1) ++ s1b)
+                     (snoc s2a0 (f, t2) ++ s2b));
+      clear hyp1; intros hyp1.
+    repeat (autodimp hyp1 h); exrepnd.
+    lsubst_tac.
+    apply member_if_inhabited in hyp1.
+    apply tequality_mkc_member_implies_equality in hyp0; eauto 2 with nequality.
+    apply sim2 in hyp0.
+
+    repeat (lsubstc_subst_aeq2;[]).
+    repeat (substc_lsubstc_vars3;[]).
+    repeat (lsubstc_weak;[]).
+    proof_irr; auto.
+
+    eexists; eexists; eexists; eexists; dands;
+      try (complete (spcast; apply computes_to_valc_refl; eauto 3 with slow));
+      repeat (lsubstc_subst_aeq2;[]);
+      repeat (substc_lsubstc_vars3;[]);
+      repeat (lsubstc_weak;[]);
+      proof_irr; auto;
+      eauto 3 with nequality.
+  }
+
+  (* conclusion *)
+
+  lsubst_tac; sp.
+
+  (*assert (wf_term (@mk_axiom p)) as wfax by eauto 2 with slow.*)
+
+  assert (wf_term (mk_prefl (mk_apply (mk_var f) a) (mk_apply (mk_var f) a))) as wfapp.
+  { apply wf_prefl; dands; apply wf_apply; eauto 3 with slow. }
+
+  assert (cover_vars (mk_prefl (mk_apply (mk_var f) a) (mk_apply (mk_var f) a))
+                     (snoc s1a0 (f, t1) ++ s1b)) as covapp1.
+  { apply cover_vars_prefl; dands;
+      apply cover_vars_apply; dands; eauto 3 with slow;
+        apply cover_vars_var; rw @dom_csub_app; rw @dom_csub_snoc; simpl;
+          rw @in_app_iff; rw in_snoc; tcsp. }
+
+  assert (cover_vars (mk_prefl (mk_apply (mk_var f) a) (mk_apply (mk_var f) a))
+                     (snoc s2a0 (f, t2) ++ s2b)) as covapp2.
+  { apply cover_vars_prefl; dands;
+      apply cover_vars_apply; dands; eauto 3 with slow;
+        apply cover_vars_var; rw @dom_csub_app; rw @dom_csub_snoc; simpl;
+          rw @in_app_iff; rw in_snoc; tcsp. }
+
+  repeat (lsubstc_subst_aeq2;[]).
+  repeat (substc_lsubstc_vars3;[]).
+  repeat (lsubstc_weak;[]).
+  proof_irr; auto.
+  revert c c0.
+  lsubst_tac.
+  introv.
+
+  pose proof (lsubstc_snoc_move
+                e2
+                (snoc s1a0 (f, t1) ++ s1b)
+                []
+                z
+                (mkc_prefl
+                   (mkc_apply t1 (lsubstc a wa (snoc s1a0 (f, t1) ++ s1b) cova1))
+                   (mkc_apply t1 (lsubstc a wa (snoc s1a0 (f, t1) ++ s1b) cova1)))
+                wfce0) as xx1.
+  allrw app_nil_r.
+  allrw @dom_csub_app.
+  allrw @dom_csub_snoc.
+  allsimpl.
+  pose proof (xx1 pt0) as xx2; clear xx1.
+  autodimp xx2 hyp.
+  { apply similarity_dom in sim6; repnd.
+    rewrite sim7.
+    apply similarity_dom in sim1; repnd.
+    rewrite sim8.
+    rewrite vars_hyps_substitute_hyps; auto.
+    rw in_app_iff; rw in_snoc; intro j; repndors; tcsp.
+  }
+  exrepnd.
+  proof_irr.
+  rewrite <- xx0; clear xx0.
+
+  pose proof (lsubstc_snoc_move
+                e2
+                (snoc s2a0 (f, t2) ++ s2b)
+                []
+                z
+                (mkc_prefl (mkc_apply t2 (lsubstc a wa (snoc s2a0 (f, t2) ++ s2b) cova2))
+                           (mkc_apply t2 (lsubstc a wa (snoc s2a0 (f, t2) ++ s2b) cova2)))
+                wfce0) as xx1.
+  allrw app_nil_r.
+  allrw @dom_csub_app.
+  allrw @dom_csub_snoc.
+  allsimpl.
+  pose proof (xx1 pt3) as xx2; clear xx1.
+  autodimp xx2 hyp.
+  { apply similarity_dom in sim6; repnd.
+    rewrite sim6.
+    apply similarity_dom in sim1; repnd.
+    rewrite sim1.
+    rewrite vars_hyps_substitute_hyps; auto.
+    rw in_app_iff; rw in_snoc; intro j; repndors; tcsp.
+  }
+  exrepnd.
+  proof_irr.
+  rewrite <- xx0; clear xx0.
+
+  auto.
+Qed.
+
+(* begin hide *)
+
+Lemma rule_function_elimination_wf_true {p} :
+  forall lib (A B C a e1 e2 e3 : NTerm)
+         (f x z : NVar)
+         (H J : @barehypotheses p)
+         (i : nat),
+    rule_true lib (rule_function_elimination_wf
+                     A B C a e1 e2 e3
+                     f x z
+                     H J
+                     i).
+Proof.
+  introv.
+  apply rule_true3_implies_rule_true.
+  apply rule_function_elimination_wf_true3.
+Qed.
+
+Lemma rule_function_elimination_wf_true2 {o} :
+  forall lib A B C a e1 e2 e3 f x z H J i,
+    @rule_true2 o lib (rule_function_elimination_wf A B C a e1 e2 e3 f x z H J i).
+Proof.
+  intros.
+  apply rule_true_iff_rule_true2.
+  apply rule_function_elimination_wf_true.
+Qed.
+
+Lemma rule_function_elimination_true_ex {p} :
+  forall lib (A B C a e1 e2 e3 : NTerm)
+         (f x z : NVar)
+         (H J : @barehypotheses p)
+         (i : nat),
+    rule_true_if lib (rule_function_elimination_wf
+                        A B C a e1 e2 e3
+                        f x z
+                        H J
+                        i).
+Proof.
+  intros.
+  generalize (rule_function_elimination_wf_true lib A B C a e1 e2 e3 f x z H J i); intro rt.
+  rw <- @rule_true_eq_ex in rt.
+  unfold rule_true_ex in rt; sp.
+Qed.
+
+
+(*
+
+
+===================================================
+TO FIX
+===================================================
+
+
+Lemma rule_function_elimination_wf_wf {o} :
+  forall (A B C a e1 e2 e3 : @NTerm o) f x z H J i,
+    wf_term a
+    -> covered a (snoc (vars_hyps H) f ++ vars_hyps J)
+    -> !LIn z (vars_hyps H)
+    -> !LIn z (vars_hyps J)
+    -> z <> f
+    -> wf_term e1
+    -> wf_term e3
+    -> wf_rule (rule_function_elimination_wf A B C a e1 e2 e3 f x z H J i).
+Proof.
+  introv wa cov nizH nizJ dzf we1 we3.
+
+  introv pwf m; allsimpl; repdors; subst; sp;
+  allunfold @pwf_sequent; wfseq; sp.
+
+  {
+    allrw @vswf_hypotheses_nil_eq.
+    allrw @wf_hypotheses_app; repnd.
+    allrw @wf_hypotheses_snoc; repnd.
+    allsimpl.
+    allapply @isprog_vars_implies_wf.
+    allrw <- @wf_function_iff; tcsp.
+  }
+
+  {
+    allrw @vswf_hypotheses_nil_eq.
+    allrw @wf_hypotheses_app; repnd.
+    allrw @wf_hypotheses_snoc; repnd.
+    allsimpl.
+    allapply @isprog_vars_implies_covered.
+    allrw @covered_function; repnd.
+    apply covered_snoc_app_weak.
+    apply covered_app_weak_l; auto.
+  }
+
+  {
+    allrw @vswf_hypotheses_nil_eq.
+    rw @wf_hypotheses_snoc; simpl; dands; tcsp.
+    - apply isprog_vars_member; dands.
+      + apply isprog_vars_apply; dands.
+        * apply isprog_vars_var_iff.
+          rw @vars_hyps_app.
+          rw @vars_hyps_snoc; simpl.
+          rw in_app_iff.
+          rw in_snoc; tcsp.
+        * rw @isprog_vars_iff_covered; dands; auto.
+          rw @vars_hyps_app.
+          rw @vars_hyps_snoc; simpl; auto.
+      + apply isprog_vars_subst2; auto.
+        * allrw @wf_hypotheses_app; repnd.
+          allrw @wf_hypotheses_snoc; repnd.
+          allsimpl.
+          allapply @isprog_vars_implies_wf.
+          allrw <- @wf_function_iff; tcsp.
+        * rw @isprog_vars_iff_covered; dands; auto.
+          rw @vars_hyps_app.
+          rw @vars_hyps_snoc; simpl; auto.
+        * allrw @wf_hypotheses_app; repnd.
+          allrw @wf_hypotheses_snoc; repnd.
+          allsimpl.
+          allrw <- @isprog_vars_function_iff; repnd.
+          allrw @vars_hyps_app.
+          allrw @vars_hyps_snoc; simpl.
+          eapply isprog_vars_subvars;[|eauto].
+          rw subvars_eq; introv i; allsimpl.
+          allrw in_app_iff; allrw in_snoc; tcsp.
+    - intro i.
+      allrw @vars_hyps_app.
+      allrw @vars_hyps_snoc; allsimpl.
+      allrw in_app_iff; allrw in_snoc.
+      repndors; tcsp.
+  }
+
+  {
+    allrw @wf_term_eq.
+    allrw @nt_wf_lsubst_iff; tcsp.
+  }
+
+  {
+    apply covered_snoc_weak; auto.
+  }
+Qed.
+
+Lemma rule_function_elimination_wf_wf2 {o} :
+  forall (A B C a e1 e2 e3 : @NTerm o) f x z H J i,
+    wf_term a
+    -> covered a (snoc (vars_hyps H) f ++ vars_hyps J)
+    -> !LIn z (vars_hyps H)
+    -> !LIn z (vars_hyps J)
+    -> z <> f
+    -> wf_rule2 (rule_function_elimination_wf A B C a e1 e2 e3 f x z H J i).
+Proof.
+  introv wa cova nizH nizJ dzf wf j.
+  allsimpl; repndors; subst; tcsp;
+  allunfold @wf_bseq; repnd; allsimpl; wfseq.
+
+  - allrw @vswf_hypotheses_nil_eq.
+    allrw @wf_hypotheses_app; repnd.
+    allrw @wf_hypotheses_snoc; repnd.
+    allapply @isprog_vars_implies_wf.
+    allrw <- @wf_function_iff; tcsp.
+
+  - allrw @vswf_hypotheses_nil_eq.
+    allrw @wf_hypotheses_app; repnd.
+    allrw @wf_hypotheses_snoc; repnd.
+    allapply @isprog_vars_implies_covered.
+    allrw @covered_function; repnd.
+    apply covered_snoc_app_weak.
+    apply covered_app_weak_l; auto.
+
+  - allrw @vswf_hypotheses_nil_eq.
+    rw @wf_hypotheses_snoc; simpl; dands; tcsp.
+    { apply isprog_vars_member; dands.
+      + apply isprog_vars_apply; dands.
+        * apply isprog_vars_var_iff.
+          rw @vars_hyps_app.
+          rw @vars_hyps_snoc; simpl.
+          rw in_app_iff.
+          rw in_snoc; tcsp.
+        * rw @isprog_vars_iff_covered; dands; auto.
+          rw @vars_hyps_app.
+          rw @vars_hyps_snoc; simpl; auto.
+      + apply isprog_vars_subst2; auto.
+        * allrw @wf_hypotheses_app; repnd.
+          allrw @wf_hypotheses_snoc; repnd.
+          allsimpl.
+          allapply @isprog_vars_implies_wf.
+          allrw <- @wf_function_iff; tcsp.
+        * rw @isprog_vars_iff_covered; dands; auto.
+          rw @vars_hyps_app.
+          rw @vars_hyps_snoc; simpl; auto.
+        * allrw @wf_hypotheses_app; repnd.
+          allrw @wf_hypotheses_snoc; repnd.
+          allsimpl.
+          allrw <- @isprog_vars_function_iff; repnd.
+          allrw @vars_hyps_app.
+          allrw @vars_hyps_snoc; simpl.
+          eapply isprog_vars_subvars;[|eauto].
+          rw subvars_eq; introv i; allsimpl.
+          allrw in_app_iff; allrw in_snoc; tcsp.
+    }
+    { intro i.
+      allrw @vars_hyps_app.
+      allrw @vars_hyps_snoc; allsimpl.
+      allrw in_app_iff; allrw in_snoc.
+      repndors; tcsp.
+    }
+
+  - apply covered_snoc_weak; auto.
+Qed.
+*)
+
+
+
+XXXXXXXXXXXXXXXXXXXX
+
+
+
+(* [25] ============ LAMBDA EQUALITY ============ *)
+
+(**
+
+  The following rule is called the lambda equality rule.  It allows
+  one to prove that lambda-abstractions are well-typed.
+<<
+
+   H |- \x1.t1 = \x2.t2 in x:A->B
+
+     By lambdaEquality lvl(i) z ()
+
+     H z : A |- t1[x1\z] = t2[x2\z] in B[x\z]
+     H |- A = A in Type(i)
+>>
+ *)
+
+(* NOTE: if we could destruct prefl terms, then we could essentially return the
+   extract mk_prefl(\z.pi1(e1), \z.pi2(e1)) here,
+   where pi1/pi2 here gets the first/second component of a prefl term.
+ *)
+
+Definition rule_lambda_equality {o}
+           (A B t1 t2 e1 e2 : NTerm)
+           (x1 x2 x z : NVar)
+           (i : nat)
+           (H : @barehypotheses o) :=
+  mk_rule
+    (mk_baresequent
+       H
+       (mk_concl_eq (mk_lam x1 t1)
+                    (mk_lam x2 t2)
+                    (mk_function A x B)))
+    [ mk_baresequent
+        (snoc H (mk_hyp z A))
+        (mk_concl_eq_ext (subst t1 x1 (mk_var z))
+                         (subst t2 x2 (mk_var z))
+                         (subst B x (mk_var z))
+                         e1),
+      mk_baresequent
+        H
+        (mk_concl_eq_ext A A (mk_uni i) e2) ]
+    [ sarg_var z , sarg_term (mk_lam x1 t1) ].
+
+Lemma rule_lambda_equality_true {o} :
+  forall lib (A B t1 t2 e1 e2 : NTerm)
+         (x1 x2 x z : NVar)
+         (i   : nat)
+         (H   : @barehypotheses o)
+         (bc1 : !LIn z (bound_vars B))
+         (bc2 : !LIn z (bound_vars t1))
+         (bc3 : !LIn z (bound_vars t2)),
+    rule_true lib (rule_lambda_equality A B t1 t2 e1 e2 x1 x2 x z i H).
+Proof.
+  intros.
+  unfold rule_lambda_equality, rule_true, closed_type_baresequent, closed_extract_baresequent; simpl.
+  intros.
+
+  pose proof (cargs (sarg_term (mk_lam x1 t1))) as carg1; simpl in carg1; autodimp carg1 hyp.
+  clear cargs.
+
+  (* We prove the well-formedness of things *)
+  destseq; allsimpl.
+  dLin_hyp; exrepnd.
+  rename Hyp0 into hyp1; rename Hyp1 into hyp2.
+  destseq; allsimpl; proof_irr; GC.
+
+  allunfold @closed_type; allunfold @closed_extract; allsimpl.
+  duplicate wfct as wfi.
+  rw <- @wf_equality_iff in wfct.
+  destruct wfct as [ wl1 wfct ].
+  destruct wfct as [ wl2 wfct ].
+  rw <- @wf_function_iff in wfct.
+  destruct wfct as [ wA wB ].
+  duplicate ce0 as ce.
+  allrw @nh_vars_hyps_snoc; allsimpl.
+
+  match goal with
+  | [ |- context[covered ?a ?b] ] => assert (covered a b) as covc
+  end.
+  {
+    clear hyp1 hyp2.
+    apply covered_prefl_same; auto.
+  }
+  exists covc.
+
+  (* We prove some simple facts on our sequents *)
+  assert ((z <> x -> !LIn z (free_vars B))
+          # (z <> x1 -> !LIn z (free_vars t1))
+          # (z <> x2 -> !LIn z (free_vars t2))
+          # !LIn z (free_vars A)
+          # !LIn z (vars_hyps H)) as vhyps.
+
+  {
+    clear hyp1 hyp2.
+    dwfseq.
+    sp;
+      try (complete (generalize (cg z); sp;
+                     allrw in_remove_nvars; allsimpl;
+                     autodimp X0 h; sp));
+      try (complete (generalize (cg0 z); sp;
+                     allrw in_remove_nvars; allsimpl;
+                     autodimp X0 h; sp));
+      try (complete (generalize (cg1 z); sp;
+                     allrw in_remove_nvars; allsimpl;
+                     autodimp X0 h; sp));
+      try (complete (apply_in_hyp p;
+                     generalize (subvars_hs_vars_hyps H); intro sv;
+                     rw subvars_prop in sv;
+                     apply sv in p; sp)).
+  }
+
+  destruct vhyps as [ nzB vhyps ].
+  destruct vhyps as [ nzt1 vhyps ].
+  destruct vhyps as [ nzt2 vhyps ].
+  destruct vhyps as [ nzA nzH ].
+  (* done with proving these simple facts *)
+
+  (* we now start proving the sequent *)
+  vr_seq_true.
+
+  lsubst_tac.
+
+  pose proof (teq_and_eq_if_equality2
+                lib
+                (mk_function A x B) (mk_lam x1 t1) (mk_lam x2 t2) s1 s2 H
+                wT wl1 wl2 c1 c0 c2 c3 cT cT0 eqh sim) as k.
+  lsubst_tac.
+  apply k; clear k.
+
+  {
+    
+  }
+
+  rw @tequality_function.
+
+  split.
+
+  (* First, we prove that the a's are types *)
+  vr_seq_true in hyp2.
+  generalize (hyp2 s1 s2 eqh sim); clear hyp2; intro hyp2; exrepnd.
+  lsubst_tac.
+  rw @member_eq in hyp2.
+  rw <- @member_equality_iff in hyp2.
+  apply @equality_commutes2 in hyp0; try (complete auto).
+  apply @equality_in_uni in hyp0; auto.
+
+  (* Then we prove that the b's are type families *)
+  intros a a' ea.
+  vr_seq_true in hyp1.
+  generalize (hyp1 (snoc s1 (z, a)) (snoc s2 (z, a'))); clear hyp1; intro hyp1.
+  autodimp hyp1 hyp.
+
+  (* we have to prove the functionality of our hypotheses *)
+  apply hyps_functionality_snoc2; simpl; try (complete sp).
+  introv eq s.
+  vr_seq_true in hyp2.
+  generalize (hyp2 s1 s' eqh s); clear hyp2; intro hyp2; exrepnd.
+  lsubst_tac.
+  rw @member_eq in hyp1.
+  rw <- @member_equality_iff in hyp1.
+  apply @equality_commutes2 in hyp0; try (complete auto).
+  apply @equality_in_uni in hyp0; auto.
+
+  (* we have to prove the similarity of our hypotheses *)
+  autodimp hyp1 hyp.
+  rw @similarity_snoc; simpl.
+  exists s1 s2 a a' wA c4; sp.
+
+  (* we can now use hyp1 *)
+  exrepnd; lsubst_tac.
+
+  (* we use hyp0 *)
+  rw @tequality_mkc_equality2_sp in hyp0; repnd.
+
+  (* we use hyp3 *)
+  assert (lsubstc (subst B x (mk_var z)) wT0 (snoc s1 (z, a)) cT1
+          = substc a x (lsubstc_vars B wB (csub_filter s1 [x]) [x] c5)) as eq1
+         by (apply lsubstc_subst_snoc_eq; try (complete sp);
+             allapply @similarity_dom; exrepd; allrw; sp).
+
+  rewrite eq1 in hyp3.
+
+  assert (lsubstc (subst B x (mk_var z)) wT0 (snoc s2 (z, a')) cT2
+          = substc a' x (lsubstc_vars B wB (csub_filter s2 [x]) [x] c7)) as eq2
+         by (apply lsubstc_subst_snoc_eq; try (complete sp);
+             allapply @similarity_dom; exrepd; allrw; sp).
+
+  rewrite eq2 in hyp3.
+
+  sp.
+
+
+  (* we prove the membership *)
+  clear dependent s1; clear dependent s2.
+  introv hf sim.
+  lsubst_tac.
+  rw @equality_in_function3.
+
+  dands.
+
+  vr_seq_true in hyp2.
+  generalize (hyp2 s1 s2 hf sim); clear hyp2; intro hyp2; exrepnd.
+  lsubst_tac.
+  rw @member_eq in hyp2.
+  rw <- @member_equality_iff in hyp2.
+  apply @equality_in_uni in hyp2; auto.
+
+  introv ea.
+
+  assert (cover_vars (mk_var z) (snoc s1 (z, a)))
+    as cv1 by (apply @cover_vars_var; rw @dom_csub_snoc; simpl; rw in_snoc; sp).
+
+  assert (cover_vars (mk_var z) (snoc s2 (z, a')))
+    as cv2 by (apply @cover_vars_var; rw @dom_csub_snoc; simpl; rw in_snoc; sp).
+
+  assert (disjoint (free_vars (@mk_var o z)) (bound_vars t1))
+    as disj1 by (simpl; rw disjoint_singleton_l; sp).
+
+  assert (disjoint (free_vars (@mk_var o z)) (bound_vars t2))
+    as disj2 by (simpl; rw disjoint_singleton_l; sp).
+
+  assert (disjoint (free_vars (@mk_var o z)) (bound_vars B))
+    as disjB by (simpl; rw disjoint_singleton_l; sp).
+
+  dands.
+
+  vr_seq_true in hyp1.
+  generalize (hyp1 (snoc s1 (z, a)) (snoc s1 (z, a'))); clear hyp1; intro hyp1.
+  autodimp hyp1 hyp.
+
+  (* we have to prove the functionality of our hypotheses *)
+  apply hyps_functionality_snoc2; simpl; try (complete sp).
+  introv eq sim'.
+  vr_seq_true in hyp2.
+  generalize (hyp2 s1 s' hf sim'); clear hyp2; intro hyp2; exrepd.
+  lsubst_tac.
+  rw @member_eq in e.
+  rw <- @member_equality_iff in e.
+  apply @equality_commutes2 in t; try (complete auto).
+  apply @equality_in_uni in t; auto.
+
+  (* we have to prove the similarity of our hypotheses *)
+  autodimp hyp1 hyp.
+  rw @similarity_snoc; simpl.
+  exists s1 s1 a a' wA c1; sp.
+  apply @similarity_refl in sim; auto.
+
+  exrepnd.
+  lsubst_tac.
+  rw @tequality_mkc_equality2_sp in hyp0; repnd.
+  clear hyp1 hyp0.
+
+  assert (lsubstc (subst B x (mk_var z)) wT0 (snoc s1 (z, a)) cT
+          = substc a x (lsubstc_vars B wB (csub_filter s1 [x]) [x] c2)) as eq1
+         by (apply lsubstc_subst_snoc_eq; try (complete sp);
+             allapply @similarity_dom; exrepd; allrw; sp).
+
+  rewrite eq1 in hyp3; clear eq1.
+
+  assert (lsubstc (subst B x (mk_var z)) wT0 (snoc s1 (z, a')) cT0
+          = substc a' x (lsubstc_vars B wB (csub_filter s1 [x]) [x] c2)) as eq2
+         by (apply lsubstc_subst_snoc_eq; try (complete sp);
+             allapply @similarity_dom; exrepd; allrw; sp).
+
+  rewrite eq2 in hyp3; clear eq2.
+  auto.
+
+  repeat betared.
+
+  vr_seq_true in hyp1.
+  generalize (hyp1 (snoc s1 (z, a)) (snoc s2 (z, a'))); clear hyp1; intro hyp1.
+  autodimp hyp1 hyp.
+
+  (* we have to prove the functionality of our hypotheses *)
+  apply hyps_functionality_snoc2; simpl; try (complete sp).
+  introv eq sim'.
+  vr_seq_true in hyp2.
+  generalize (hyp2 s1 s' hf sim'); clear hyp2; intro hyp2; exrepd.
+  lsubst_tac.
+  rw @member_eq in e.
+  rw <- @member_equality_iff in e.
+  apply @equality_commutes2 in t; try (complete auto).
+  apply @equality_in_uni in t; auto.
+
+  (* we have to prove the similarity of our hypotheses *)
+  autodimp hyp1 hyp.
+  rw @similarity_snoc; simpl.
+  exists s1 s2 a a' wA c1; sp.
+
+  exrepnd.
+  lsubst_tac.
+  rw @member_eq in hyp1.
+  rw <- @member_equality_iff in hyp1.
+
+  apply @equality_commutes4 in hyp0; auto; clear hyp1.
+
+  assert (lsubstc (subst B x (mk_var z)) wT0 (snoc s1 (z, a)) cT
+          = substc a x (lsubstc_vars B wB (csub_filter s1 [x]) [x] c2)) as eq
+         by (apply lsubstc_subst_snoc_eq; try (complete sp);
+             allapply @similarity_dom; exrepd; allrw; sp).
+
+  rewrite eq in hyp0; clear eq.
+
+  assert (lsubstc (subst t1 x1 (mk_var z)) w2 (snoc s1 (z, a)) c4
+          = substc a x1 (lsubstc_vars t1 w1 (csub_filter s1 [x1]) [x1] c0)) as eq
+         by (apply lsubstc_subst_snoc_eq; try (complete sp);
+             allapply @similarity_dom; exrepd; allrw; sp).
+
+  rewrite eq in hyp0; clear eq.
+
+  assert (lsubstc (subst t2 x2 (mk_var z)) w3 (snoc s2 (z, a')) c7
+          = substc a' x2 (lsubstc_vars t2 w0 (csub_filter s2 [x2]) [x2] c3)) as eq
+         by (apply lsubstc_subst_snoc_eq; try (complete sp);
+             allapply @similarity_dom; exrepd; allrw; sp).
+
+  rewrite eq in hyp0; clear eq.
+  auto.
+Qed.
+
+
+
+(* [26] ============ APPLY @EQUALITY ============ *)
+
+(**
+
+  We following rule called ``apply @equality`` allows one to prove that
+  applications are well-typed.
+<<
+   H |- f1 t1 = f2 t2 in B[x\t1]
+
+     By applyEquality ()
+
+     H |- f1 = f2 in x:A->B
+     H |- t1 = t2 in A
+>>
+ *)
+
+Definition rule_apply_equality {o}
+           (A B f1 f2 t1 t2 e1 e2 : NTerm)
+           (x : NVar)
+           (H : @barehypotheses o) :=
+  mk_rule
+    (mk_baresequent H (mk_concl_eq_ext (mk_apply f1 t1)
+                                       (mk_apply f2 t2)
+                                       (subst B x t1)
+                                       (mk_apply e1 e2)))
+    [ mk_baresequent H (mk_concl_eq_ext f1 f2 (mk_function A x B) e1),
+      mk_baresequent H (mk_concl_eq_ext t1 t2 A e2)
+    ]
+    [].
+
+Lemma rule_apply_equality_true {o} :
+  forall lib (A B f1 f2 t1 t2 e1 e2 : NTerm)
+         (x : NVar)
+         (i   : nat)
+         (H   : @barehypotheses o)
+         (bc1 : disjoint (free_vars t1) (bound_vars B))
+         (bc2 : disjoint (free_vars t2) (bound_vars B)),
+    rule_true lib (rule_apply_equality A B f1 f2 t1 t2 e1 e2 x H).
+Proof.
+  intros.
+  unfold rule_apply_equality, rule_true, closed_type_baresequent, closed_extract_baresequent; simpl.
+  intros.
+
+  (* We prove the well-formedness of things *)
+  destseq; allsimpl.
+  dLin_hyp; exrepnd.
+  rename Hyp0 into hyp1.
+  rename Hyp1 into hyp2.
+  destseq; allsimpl; proof_irr; GC.
+
+  allunfold @closed_type; allunfold @closed_extract; allsimpl.
+  duplicate wfct as wfi.
+  rw <- @wf_equality_iff in wfct.
+  destruct wfct as [ wa1 wfct ].
+  destruct wfct as [ wa2 wfct ].
+  rw <- @wf_apply_iff in wa1.
+  destruct wa1 as [ wf1 wt1 ].
+  rw <- @wf_apply_iff in wa2.
+  destruct wa2 as [ wf2 wt2 ].
+
+  match goal with
+  | [ |- context[covered ?a ?b] ] => assert (covered a b) as cov
+  end.
+  { apply covered_apply; dands; auto. }
+  exists cov.
+
+  (* We prove some simple facts on our sequents *)
+  (* xxx *)
+  (* done with proving these simple facts *)
+
+  (* we now start proving the sequent *)
+  vr_seq_true.
+  vr_seq_true in hyp1.
+  vr_seq_true in hyp2.
+  generalize (hyp1 s1 s2 eqh sim); clear hyp1; intro hyp1; exrepnd.
+  generalize (hyp2 s1 s2 eqh sim); clear hyp2; intro hyp2; exrepnd.
+
+  lsubst_tac.
+
+  rw @tequality_mkc_equality in hyp0; repnd.
+  rw @tequality_mkc_equality in hyp3; repnd.
+
+  rw @tequality_mkc_equality.
+
+  dands.
+
+
+
+
+
+  allrw @member_eq.
+  allrw <- @member_equality_iff.
+  rw @tequality_mkc_equality2_sp in hyp3.
+  rw @tequality_mkc_equality2_sp in hyp0.
+  rw @tequality_mkc_equality2_sp; repnd.
+  repeat (rw prod_assoc).
+  rw @tequality_function in hyp4; repnd.
+
+  allunfold @equorsq2; repnd.
+
+  (* a few assertions *)
+  assert (equality lib (lsubstc t1 wt1 s1 c1)
+                   (lsubstc t1 wt1 s2 c4)
+                   (lsubstc A wT s1 cT))
+         as eq1
+         by (apply @cequorsq_equality_trans2 with (t2 := lsubstc t1 wt1 s1 c1); sp;
+             allapply @equality_refl; sp).
+
+  assert (equality lib (lsubstc f1 wf1 s1 c0)
+                   (lsubstc f1 wf1 s2 c7)
+                   (mkc_function (lsubstc A wT s1 cT) x
+                                 (lsubstc_vars B w2 (csub_filter s1 [x]) [x] c5)))
+         as eq3
+         by (apply @cequorsq_equality_trans2 with (t2 := lsubstc f1 wf1 s1 c0); sp;
+             allapply @equality_refl; sp).
+
+  assert (equality lib (lsubstc t2 wt2 s1 c2)
+                   (lsubstc t2 wt2 s2 c6)
+                   (lsubstc A wT s1 cT))
+         as eq5
+         by (apply @cequorsq_equality_trans2 with (t2 := lsubstc t2 wt2 s1 c2); sp;
+             apply @equality_sym in hyp2; apply @equality_refl in hyp2; sp).
+
+  assert (equality lib (lsubstc f2 wf2 s1 c3)
+                   (lsubstc f2 wf2 s2 c8)
+                   (mkc_function (lsubstc A wT s1 cT) x
+                                 (lsubstc_vars B w2 (csub_filter s1 [x]) [x] c5)))
+         as eq6
+         by (apply @cequorsq_equality_trans2 with (t2 := lsubstc f2 wf2 s1 c3); sp;
+             apply @equality_sym in hyp1; apply @equality_refl in hyp1; sp).
+
+  assert (equality lib (lsubstc t1 wt1 s1 c1)
+                   (lsubstc t2 wt2 s2 c6)
+                   (lsubstc A wT s1 cT))
+         as eq7 by (apply @equality_trans with (t2 := lsubstc t2 wt2 s1 c2); sp).
+
+  assert (wf_term (subst B x t2))
+         as wfs2
+         by (apply lsubst_preserves_wf_term; sp;
+             unfold wf_sub, sub_range_sat; simpl; sp; cpx; rw @nt_wf_eq; sp).
+
+  assert (cover_vars (subst B x t2) s1)
+         as cv2.
+  (* begin proof of assert *)
+  rw @cover_vars_eq.
+  rw @cover_vars_eq in cT3.
+  unfold subst.
+  rw subvars_prop; introv k.
+  generalize (eqvars_free_vars_disjoint B [(x,t1)]); intro u1.
+  generalize (eqvars_free_vars_disjoint B [(x,t2)]); intro u2.
+  rw eqvars_prop in u1.
+  rw eqvars_prop in u2.
+  rw u2 in k; simpl in k.
+  rw in_app_iff in k; rw in_remove_nvars in k; rw in_single_iff in k; repdors; repnd.
+  rw subvars_prop in cT3.
+  apply cT3; unfold subst.
+  rw u1.
+  rw in_app_iff; rw in_remove_nvars; rw in_single_iff; sp.
+  revert k.
+  boolvar; simpl; allrw app_nil_r; intro k; sp.
+  clear_dependents c2.
+  rw @cover_vars_eq in c2.
+  rw subvars_prop in c2.
+  apply c2; sp.
+  (* end proof of assert *)
+
+  assert (cover_vars (subst B x t2) s2)
+         as cv3
+         by (rw @cover_vars_eq;
+             rw @cover_vars_eq in cv2;
+             allapply @similarity_dom; repnd; allrw;
+             rw sim0 in cv2; sp).
+
+  assert (tequality lib (lsubstc (subst B x t1) wfct s1 cT3)
+                    (lsubstc (subst B x t2) wfs2 s1 cv2)) as teqB.
+  (* begin proof of assert *)
+  generalize (hyp4 (lsubstc t1 wt1 s1 c1) (lsubstc t2 wt2 s2 c6)); intro k1.
+  autodimp k1 hyp; sp.
+  generalize (hyp4 (lsubstc t2 wt2 s1 c2) (lsubstc t2 wt2 s2 c6)); intro k2.
+  autodimp k2 hyp; sp.
+  generalize (simple_lsubstc_subst t1 x B wfct s1 cT3 wt1 c1 w2 c5); intro e1.
+  autodimp e1 hyp.
+  rw <- e1 in k1; clear e1.
+  generalize (simple_lsubstc_subst t2 x B wfs2 s1 cv2 wt2 c2 w2 c5); intro e1.
+  autodimp e1 hyp.
+  rw <- e1 in k2; clear e1.
+  generalize (simple_lsubstc_subst t2 x B wfs2 s2 cv3 wt2 c6 w2 c10); intro e1.
+  autodimp e1 hyp.
+  rw <- e1 in k1; rw <- e1 in k2; clear e1.
+  apply @tequality_trans with (t2 := lsubstc (subst B x t2) wfs2 s2 cv3); sp.
+  apply @tequality_sym; sp.
+  (* end proof of assert *)
+
+
+  (* now we start proving our conclusion *)
+  dands.
+
+  (* from hyp 4 *)
+  generalize (hyp4 (lsubstc t1 wt1 s1 c1) (lsubstc t1 wt1 s2 c4) eq1); intro teq.
+
+  generalize (simple_lsubstc_subst t1 x B wfct s1 cT3 wt1 c1 w2 c5); intro e1.
+  autodimp e1 hyp.
+  rw <- e1 in teq.
+
+  generalize (simple_lsubstc_subst t1 x B wfct s2 cT4 wt1 c4 w2 c10); intro e2.
+  autodimp e2 hyp.
+  rw <- e2 in teq; sp.
+
+  (* from eq3 and eq1 *)
+  rw @equality_in_function in eq3; repnd.
+  generalize (eq3 (lsubstc t1 wt1 s1 c1) (lsubstc t1 wt1 s2 c4) eq1); intro e'.
+  generalize (simple_lsubstc_subst t1 x B wfct s1 cT3 wt1 c1 w2 c5); intro e1.
+  autodimp e1 hyp.
+  rw <- e1 in e'; sp.
+
+  (* from eq6 and eq5 *)
+  rw @equality_in_function in eq6; repnd.
+  generalize (eq6 (lsubstc t2 wt2 s1 c2) (lsubstc t2 wt2 s2 c6) eq5); intro e'.
+  generalize (simple_lsubstc_subst t2 x B wfs2 s1 cv2 wt2 c2 w2 c5); intro e1.
+  autodimp e1 hyp.
+  rw <- e1 in e'; sp.
+  left.
+  eapply @tequality_preserving_equality.
+  exact e'.
+  apply @tequality_sym; sp.
+
+  (* from hyp1 and hyp2 *)
+  rw @equality_in_function in hyp1; repnd.
+  generalize (hyp1 (lsubstc t1 wt1 s1 c1) (lsubstc t2 wt2 s1 c2) hyp2); intro e'.
+  generalize (simple_lsubstc_subst t1 x B wfct s1 cT3 wt1 c1 w2 c5); intro e1.
+  autodimp e1 hyp.
+  rw <- e1 in e'; sp.
+Qed.
+
+
+
+
+
+
+(* begin hide *)
+
+
+
+(* end hide *)
+
+
+(* begin hide *)
+
+
+
+(* end hide *)
+
+
+(* [28] ============ FUNCTION EXTENSIONALITY ============ *)
+
+(**
+
+  The following rule called the ``function extensionality rule''
+  states that the equality between functions in Nuprl is extensional.
+<<
+   H |- f1 = f2 in x:A->B
+
+     By funcionExtensionality lvl(i) z ()
+
+     H z : A |- f1 z = f2 z in B[x\z]
+     H |- A = A in Type(i)
+>>
+ *)
+
+Definition rule_function_extensionality {o}
+           (A B f1 f2 : NTerm)
+           (x z : NVar)
+           (i : nat)
+           (H : @barehypotheses o) :=
+  mk_rule
+    (mk_baresequent
+       H
+       (mk_conclax (mk_equality f1 f2 (mk_function A x B))))
+    [ mk_baresequent
+        (snoc H (mk_hyp z A))
+        (mk_conclax (mk_equality
+                       (mk_apply f1 (mk_var z))
+                       (mk_apply f2 (mk_var z))
+                       (subst B x (mk_var z)))),
+      mk_baresequent
+        H
+        (mk_conclax (mk_equality A A (mk_uni i))) ]
+    [sarg_var z].
+
+Lemma rule_function_extensionality_true {o} :
+  forall lib (A B f1 f2 : NTerm)
+         (x z : NVar)
+         (i   : nat)
+         (H   : @barehypotheses o)
+         (bc1 : !LIn z (bound_vars B)),
+    rule_true lib (rule_function_extensionality A B f1 f2 x z i H).
+Proof.
+  intros.
+  unfold rule_function_extensionality, rule_true, closed_type_baresequent, closed_extract_baresequent; simpl.
+  intros.
+
+  (* We prove the well-formedness of things *)
+  destseq; allsimpl.
+  generalize (hyps (mk_baresequent (snoc H (mk_hyp z A))
+                                  (mk_conclax (mk_equality
+                                                 (mk_apply f1 (mk_var z))
+                                                 (mk_apply f2 (mk_var z))
+                                                 (subst B x (mk_var z)))))
+                   (inl eq_refl))
+             (hyps (mk_baresequent H (mk_conclax (mk_equality A A (mk_uni i))))
+                   (inr (inl eq_refl)));
+    simpl; intros hyp1 hyp2.
+  destruct hyp1 as [ ws1 hyp1 ].
+  destruct hyp2 as [ ws2 hyp2 ].
+  destseq; allsimpl; proof_irr; GC.
+
+  allunfold @closed_type; allunfold @closed_extract; allsimpl.
+  duplicate wfct as wfi.
+  rw <- @wf_equality_iff in wfct.
+  destruct wfct as [ wf1 wfct ].
+  destruct wfct as [ wf2 wfct ].
+  rw <- @wf_function_iff in wfct.
+  destruct wfct as [ wA wB ].
+
+  exists (@covered_axiom o (nh_vars_hyps H)); GC.
+
+  (* We prove some simple facts on our sequents *)
+  assert ((z <> x -> !LIn z (free_vars B))
+          # !LIn z (free_vars f1)
+          # !LIn z (free_vars f2)
+          # !LIn z (free_vars A)
+          # !LIn z (vars_hyps H)) as vhyps.
+
+  clear hyp1 hyp2.
+  dwfseq.
+  sp;
+  try (complete (generalize (cg z); sp;
+                 allrw in_remove_nvars; allsimpl;
+                 autodimp X0 h; sp));
+  try (complete (generalize (cg0 z); sp;
+                 allrw in_remove_nvars; allsimpl;
+                 autodimp X0 h; sp));
+  try (complete (generalize (cg1 z); sp;
+                 allrw in_remove_nvars; allsimpl;
+                 autodimp X0 h; sp));
+  try (complete (apply_in_hyp p;
+                 generalize (subvars_hs_vars_hyps H); intro sv;
+                 rw subvars_prop in sv;
+                 apply sv in p; sp)).
+
+  destruct vhyps as [ nzB  vhyps ].
+  destruct vhyps as [ nzf1 vhyps ].
+  destruct vhyps as [ nzf2 vhyps ].
+  destruct vhyps as [ nzA  nzH ].
+  (* done with proving these simple facts *)
+
+  (* we now start proving the sequent *)
+  vr_seq_true.
+
+  lift_lsubst.
+  rw @member_eq.
+  rw <- @member_equality_iff.
+
+  assert (tequality lib
+            (mkc_function (lsubstc A wA s1 c4) x
+                          (lsubstc_vars B wB (csub_filter s1 [x]) [x] c5))
+            (mkc_function (lsubstc A wA s2 c6) x
+                          (lsubstc_vars B wB (csub_filter s2 [x]) [x] c7))) as eqfunc.
+
+  rw @tequality_function.
+
+  split.
+
+  (* First, we prove that the a's are types *)
+  vr_seq_true in hyp2.
+  generalize (hyp2 s1 s2 eqh sim); clear hyp2; intro hyp2.
+  exrepd.
+  lift_lsubst in t.
+  lift_lsubst in e.
+  rw @member_eq in e.
+  rw <- @member_equality_iff in e.
+  applydup @equality_in_uni in e as e'.
+  rw @fold_type in e'.
+  apply @equality_commutes2 in t; try (complete auto).
+  apply @equality_in_uni in t; sp.
+
+  (* Then we prove that the b's are type families *)
+  intros a a' eqaa'.
+  vr_seq_true in hyp1.
+  generalize (hyp1 (snoc s1 (z, a)) (snoc s2 (z, a'))); clear hyp1; intro hyp1.
+  autodimp hyp1 hyp.
+
+  (* we have to prove the functionality of our hypotheses *)
+  apply hyps_functionality_snoc2; simpl; try (complete sp).
+  introv eq s.
+  vr_seq_true in hyp2.
+  generalize (hyp2 s1 s' eqh s); clear hyp2; intro hyp2.
+  exrepd.
+  lift_lsubst in t.
+  lift_lsubst in e.
+  rw @member_eq in e.
+  rw <- @member_equality_iff in e.
+  applydup @equality_in_uni in e as e'.
+  rw @fold_type in e'.
+  apply @equality_commutes2 in t; try (complete auto).
+  apply @equality_in_uni in t; sp.
+
+  (* we have to prove the similarity of our hypotheses *)
+  autodimp hyp1 hyp.
+  rw @similarity_snoc; simpl.
+  exists s1 s2 a a' wA c4; sp.
+
+  (* we can now use hyp1 *)
+  exrepnd; lsubst_tac.
+
+  (* we use hyp0 *)
+  rw @tequality_mkc_equality2_sp in hyp0; repnd.
+
+  (* we use hyp3 *)
+  assert (lsubstc (subst B x (mk_var z)) wT0 (snoc s1 (z, a)) cT1
+          = substc a x (lsubstc_vars B wB (csub_filter s1 [x]) [x] c5)) as eq1
+         by (apply lsubstc_subst_snoc_eq; try (complete sp);
+             allapply @similarity_dom; exrepd; allrw; sp).
+
+  rewrite eq1 in hyp3.
+
+  assert (lsubstc (subst B x (mk_var z)) wT0 (snoc s2 (z, a')) cT2
+          = substc a' x (lsubstc_vars B wB (csub_filter s2 [x]) [x] c7)) as eq2
+         by (apply lsubstc_subst_snoc_eq; try (complete sp);
+             allapply @similarity_dom; exrepd; allrw; sp).
+
+  rewrite eq2 in hyp3.
+
+  sp.
+
+
+  (* we prove the membership *)
+  assert (forall a a' s1 s2,
+            hyps_functionality lib s1 H
+            -> similarity lib s1 s2 H
+            -> {c1f : cover_vars f1 s1
+                , {c2f : cover_vars f2 s2
+                , {c1A : cover_vars A s1
+                , {c1B : cover_vars_upto B (csub_filter s1 [x]) [x]
+                , equality lib a a' (lsubstc A wA s1 c1A)
+                  -> equality lib
+                       (mkc_apply (lsubstc f1 wf1 s1 c1f) a)
+                       (mkc_apply (lsubstc f2 wf2 s2 c2f) a')
+                       (substc a x (lsubstc_vars B wB (csub_filter s1 [x]) [x] c1B))}}}}) as eqlam.
+  introv eqh0 sim0.
+
+  assert (cover_vars f1 s0) as c1f1.
+  clear eqfunc.
+  allapply @similarity_dom; repnd.
+  allrw @cover_vars_eq.
+  allrw.
+  rw sim2 in c1; sp.
+
+  assert (cover_vars f1 s3) as c2f1.
+  clear eqfunc.
+  allapply @similarity_dom; repnd.
+  allrw @cover_vars_eq.
+  allrw.
+  rw sim2 in c1; sp.
+
+  assert (cover_vars f2 s0) as c1f2.
+  clear eqfunc.
+  allapply @similarity_dom; repnd.
+  allrw @cover_vars_eq.
+  allrw.
+  rw sim2 in c2; sp.
+
+  assert (cover_vars f2 s3) as c2f2.
+  clear eqfunc.
+  allapply @similarity_dom; repnd.
+  allrw @cover_vars_eq.
+  allrw.
+  rw sim2 in c2; sp.
+
+  assert (cover_vars_upto B (csub_filter s0 [x]) [x]) as cB0.
+  clear eqfunc.
+  allapply @similarity_dom; repnd.
+  allunfold @cover_vars_upto.
+  allrw @dom_csub_csub_filter.
+  allrw.
+  rw sim in c7; sp.
+
+  assert (cover_vars_upto B (csub_filter s3 [x]) [x]) as cB3.
+  clear eqfunc.
+  allapply @similarity_dom; repnd.
+  allunfold @cover_vars_upto.
+  allrw @dom_csub_csub_filter.
+  allrw.
+  rw sim in c7; sp.
+
+  assert (cover_vars A s0) as cA0.
+  clear eqfunc.
+  allrw @cover_vars_eq.
+  allapply @similarity_dom; repnd.
+  allrw.
+  rw sim in c6; sp.
+
+  assert (cover_vars A s3) as cA3.
+  clear eqfunc.
+  allrw @cover_vars_eq.
+  allapply @similarity_dom; repnd.
+  allrw.
+  rw sim in c6; sp.
+
+  exists c1f1 c2f2 cA0 cB0.
+  introv eqaa'.
+
+  vr_seq_true in hyp1.
+  generalize (hyp1 (snoc s0 (z, a)) (snoc s3 (z, a'))); clear hyp1; intro hyp1.
+  autodimp hyp1 hyp.
+
+  (* we have to prove the functionality of our hypotheses *)
+  apply hyps_functionality_snoc2; simpl; try (complete sp).
+  introv eq s.
+  vr_seq_true in hyp2.
+  generalize (hyp2 s0 s' eqh0 s); clear hyp2; intro hyp2.
+  exrepd.
+  lift_lsubst in t.
+  lift_lsubst in e.
+  rw @member_eq in e.
+  rw <- @member_equality_iff in e.
+  applydup @equality_in_uni in e as e'.
+  rw @fold_type in e'.
+  apply @equality_commutes2 in t; try (complete auto).
+  apply @equality_in_uni in t; sp.
+
+  (* we have to prove the similarity of our hypotheses *)
+  autodimp hyp1 hyp.
+  rw @similarity_snoc; simpl.
+  exists s0 s3 a a' wA cA0; sp.
+
+  (* we can now use hyp1 *)
+  exrepnd; lsubst_tac.
+  rw @tequality_mkc_equality2_sp in hyp0; repnd.
+  rw @member_eq in hyp1.
+  rw <- @member_equality_iff in hyp1.
+  clear_irr; GC.
+
+  assert (lsubstc (subst B x (mk_var z)) wT0 (snoc s0 (z, a)) cT1
+          = substc a x (lsubstc_vars B wB (csub_filter s0 [x]) [x] cB0)) as eq1
+         by (apply lsubstc_subst_snoc_eq; try (complete sp);
+             allapply @similarity_dom; exrepd; allrw; sp).
+
+  rewrite eq1 in hyp0.
+  rewrite eq1 in hyp1.
+  rewrite eq1 in hyp3.
+  clear eq1.
+
+  assert (lsubstc (subst B x (mk_var z)) wT0 (snoc s3 (z, a')) cT2
+          = substc a' x (lsubstc_vars B wB (csub_filter s3 [x]) [x] cB3)) as eq2
+         by (apply lsubstc_subst_snoc_eq; try (complete sp);
+             allapply @similarity_dom; exrepd; allrw; sp).
+
+  rewrite eq2 in hyp3.
+  clear eq2.
+
+  apply @cequorsq2_prop in hyp0; try (complete auto).
+
+  (* a few useful assertions *)
+  assert (similarity lib s1 s1 H)
+         as sim1
+         by (allapply @similarity_refl; sp).
+  assert (similarity lib s2 s2 H)
+         as sim2
+         by (apply @similarity_sym in sim; allapplydup @similarity_refl; sp;
+             apply eqh in sim; sp).
+  assert (hyps_functionality lib s2 H)
+         as eqh2
+         by (apply @similarity_hyps_functionality_trans with (s1 := s1); sp).
+
+
+  (* we start proving our conclusion *)
+  rw @equality_in_function2.
+  dands; try (complete sp).
+
+
+  (* tequality *)
+  rw @tequality_mkc_equality2_sp.
+  dands; try (complete sp).
+
+  (* we prove cequorsq2 *)
+  split.
+
+  (* application in B *)
+  left.
+  rw @equality_in_function2.
+  split; try (complete (apply @tequality_refl in eqfunc; sp)).
+  introv e.
+  assert (equality lib a' a' (lsubstc A wA s2 c6))
+         as e'
+         by (apply @equality_sym in e; apply @equality_refl in e;
+             rw @tequality_function in eqfunc; repnd;
+             eapply @tequality_preserving_equality;
+             try (exact e); sp).
+
+  generalize (eqlam a a' s1 s2 eqh sim); intro k1; exrepnd; clear_irr; sp.
+  generalize (eqlam a' a' s2 s2 eqh2 sim2); intro k2; exrepnd; clear_irr; sp.
+
+  eapply @equality_trans; sp.
+  exact k1.
+  apply @equality_sym.
+  eapply @tequality_preserving_equality.
+  exact k2.
+  apply @tequality_sym.
+  rw @tequality_function in eqfunc; repnd; sp.
+
+  (* application in B *)
+  left.
+  rw @equality_in_function2.
+  split; try (complete (apply @tequality_refl in eqfunc; sp)).
+  introv e.
+  assert (equality lib a a (lsubstc A wA s1 c4)) as e' by (allapply @equality_refl; sp).
+
+  generalize (eqlam a a' s1 s2 eqh sim); intro k1; exrepnd; clear_irr; sp.
+  generalize (eqlam a a s1 s1 eqh sim1); intro k2; exrepnd; clear_irr; sp.
+
+  eapply @equality_trans; sp.
+  apply equality_sym.
+  exact k2.
+  auto.
+
+
+  (* type *)
+  apply @tequality_refl in eqfunc; sp.
+
+
+  (* application in B *)
+  introv e.
+  generalize (eqlam a a' s1 s1 eqh sim1); intro k; exrepnd; clear_irr; sp.
+Qed.
+
+
+
+(* [17] ============ FUNCTION ELIMINATION ============ *)
+
+(**
+
+ The following rule is called the function elimination rules.  It says
+ that if we can prove that [a] is in the domain [A] then we can assume
+ that [f a] is in [B[x\a]].  As for the other rules, first we show an
+ informal statement of this rule, then we show its formal statement (a
+ [Definition]), and finally we show the statement that the rule is
+ true (a [Lemma]).  In such informal statements, we write ``C ext e''
+ to indicate that e is the extract of the sequent, i.e., the evidence
+ that C is true.  We omit the ``ext e'' part when e is [mk_axiom].
+
+<<
+   H, f : x:A->B[x], J |- C ext e[z\(f a)]
+
+     By functionElimination s z
+
+     H, f : x:A->B[x], J |- a in A
+     H, f : x:A->B[x], J, z : (f a) in B[a] |- C ext e
+>>
+
+ *)
+
+Definition rule_function_elimination_concl {o}
+           (A : @NTerm o) B C a e f x z H J :=
+  mk_baresequent
+    (snoc H (mk_hyp f (mk_function A x B)) ++ J)
+    (mk_concl C (subst e z (mk_apply (mk_var f) a))).
+
+Definition rule_function_elimination_hyp1 {o}
+           (A : @NTerm o) B a ea f x H J :=
+  mk_baresequent
+    (snoc H (mk_hyp f (mk_function A x B)) ++ J)
+    (mk_concl (mk_member a A) ea).
+
+Definition rule_function_elimination_hyp2 {o}
+           (A : @NTerm o) B C a e f x z H J :=
+  mk_baresequent
+    (snoc (snoc H (mk_hyp f (mk_function A x B)) ++ J)
+          (mk_hyp z (mk_member (mk_apply (mk_var f) a)
+                               (subst B x a))))
+    (mk_concl C e).
+
+Definition rule_function_elimination {p}
+           (A B C a e : NTerm) ea
+           (f x z : NVar)
+           (H J : @barehypotheses p) :=
+  mk_rule
+    (rule_function_elimination_concl A B C a e f x z H J)
+    [
+      rule_function_elimination_hyp1 A B a ea f x H J,
+      rule_function_elimination_hyp2 A B C a e f x z H J
+    ]
+    [ sarg_term a (*, sarg_var z*)].
+
+Lemma rule_function_elimination_true3 {p} :
+  forall lib (A B C a e : NTerm) ea
+         (f x z : NVar)
+         (H J : @barehypotheses p),
+    rule_true3 lib (rule_function_elimination
+                      A B C a e
+                      ea
+                      f x z
+                      H J).
+Proof.
+  unfold rule_function_elimination, rule_true3, wf_bseq, closed_type_baresequent, closed_extract_baresequent; simpl.
+  intros; repnd.
+
+  pose proof (cargs (sarg_term a)) as ca.
+  simpl in ca; autodimp ca hyp.
+  rw @nh_vars_hyps_app in ca; simpl in ca.
+  rw @nh_vars_hyps_snoc in ca; simpl in ca.
+
+  (* We prove the well-formedness of things *)
+  destseq; allsimpl.
+  dLin_hyp; exrepnd.
+  rename Hyp into hyp1.
+  rename Hyp0 into hyp2.
+  destruct hyp1 as [ ws1 hyp1 ].
+  destruct hyp2 as [ ws2 hyp2 ].
+  destseq; allsimpl; proof_irr; GC.
+
+  assert (wf_csequent (rule_function_elimination_concl A B C a e f x z H J)) as wfc.
+  {
+    clear hyp1 hyp2.
+    unfold wf_csequent, closed_type, closed_extract, wf_sequent, wf_concl; simpl.
+    prove_seq; eauto 3 with slow.
+    { apply wf_term_subst; eauto 3 with slow.
+      apply wf_apply; eauto 2 with slow. }
+    apply covered_subst; eauto 2 with slow.
+    { eapply covered_subvars;[|eauto].
+      autorewrite with slow; simpl.
+      rw subvars_eq; introv i; simpl.
+      repeat (allrw @in_snoc; allrw @in_app_iff).
+      repndors; tcsp. }
+    { apply covered_apply; dands; eauto 3 with slow.
+      apply covered_var; rw in_app_iff; rw in_snoc; tcsp. }
+  }
+  exists wfc.
+  unfold wf_csequent, wf_sequent, wf_concl in wfc; allsimpl; repnd; proof_irr; GC.
+
+  (* We prove some simple facts on our sequents *)
+  assert (disjoint (free_vars A) (vars_hyps J)
+          # disjoint (remove_nvars [x] (free_vars B)) (vars_hyps J)
+          # subvars (free_vars a) (snoc (vars_hyps H) f ++ vars_hyps J)
+          # wf_term a
+          # !LIn z (free_vars C)
+          # !LIn z (vars_hyps H)
+          # !LIn z (vars_hyps J)
+          # (z <> f)
+          # !LIn f (vars_hyps H)
+          # !LIn f (vars_hyps J)
+          # !LIn f (free_vars A)
+          # (x <> f -> !LIn f (free_vars B))) as vhyps.
+  {
+    clear hyp1 hyp2.
+    dwfseq.
+    sp;
+      try (complete (introv i; discover; allunfold @disjoint; discover; auto));
+      try (complete (assert (LIn f (remove_nvars [x] (free_vars B)))
+                      by (rw in_remove_nvars; rw in_single_iff; sp);
+                     discover; auto));
+      try (complete (apply wf_member_iff in wfct0; sp));
+      try (complete (generalize (wfh10 z); rw in_app_iff; rw in_snoc; sp));
+      try (complete (generalize (wfh10 f); rw in_remove_nvars; simpl; intro i;
+                     dest_imp i hyp));
+      try complete (pose proof (wfc1 z) as xx; autodimp xx hyp;
+                    rw in_app_iff in xx; rw in_snoc in xx; repndors; tcsp).
+  }
+
+  destruct vhyps as [ daj vhyps ].
+  destruct vhyps as [ dbj vhyps ].
+  destruct vhyps as [ sva vhyps ].
+  destruct vhyps as [ wa vhyps ].
+  destruct vhyps as [ nizc vhyps ].
+  destruct vhyps as [ nizh vhyps ].
+  destruct vhyps as [ nizj vhyps ].
+  destruct vhyps as [ nzf vhyps ].
+  destruct vhyps as [ nifh vhyps ].
+  destruct vhyps as [ nifj vhyps ].
+  destruct vhyps as [ nifa nifb ].
+  (* done with proving these simple facts *)
+
+  vr_seq_true.
+
+  duplicate sim as simapp.
+
+  rw @similarity_app in sim; simpl in sim; exrepnd; subst; cpx.
+  rw @similarity_snoc in sim5; simpl in sim5; exrepnd; subst; cpx.
+  lsubst_tac.
+  rw @equality_in_function in sim2; repnd.
+
+  vr_seq_true in hyp2.
+
+  assert (cover_vars a (snoc s1a0 (f, t1) ++ s1b)) as cova1.
+  {
+    apply cover_vars_eq.
+    rw @dom_csub_app; rw @dom_csub_snoc; simpl.
+    clear hyp1; revert ct0.
+    unfold covered; simpl; autorewrite with slow.
+    repeat (rw @subvars_app_l).
+    introv h; repnd; clear h; GC.
+    rw @vars_hyps_app in h0; rw @vars_hyps_snoc in h0; simpl in h0.
+    apply similarity_dom in sim6; repnd; allrw.
+    apply similarity_dom in sim1; repnd; allrw.
+    autorewrite with slow; auto.
+  }
+
+  assert (cover_vars a (snoc s2a0 (f, t2) ++ s2b)) as cova2.
+  {
+    apply cover_vars_eq.
+    rw @dom_csub_app; rw @dom_csub_snoc; simpl.
+    clear hyp1; revert ct0.
+    unfold covered; simpl; autorewrite with slow.
+    repeat (rw @subvars_app_l).
+    introv h; repnd; clear h; GC.
+    rw @vars_hyps_app in h0; rw @vars_hyps_snoc in h0; simpl in h0.
+    apply similarity_dom in sim6; repnd; allrw.
+    apply similarity_dom in sim1; repnd; allrw.
+    autorewrite with slow; auto.
+  }
+
+  generalize (hyp2 (snoc (snoc s1a0 (f, t1) ++ s1b)
+                         (z, mkc_prefl (mkc_apply t1 (lsubstc a wa (snoc s1a0 (f, t1) ++ s1b) cova1))
+                                       (mkc_apply t1 (lsubstc a wa (snoc s1a0 (f, t1) ++ s1b) cova1))))
+                   (snoc (snoc s2a0 (f, t2) ++ s2b)
+                         (z, mkc_prefl (mkc_apply t2 (lsubstc a wa (snoc s2a0 (f, t2) ++ s2b) cova2))
+                                       (mkc_apply t2 (lsubstc a wa (snoc s2a0 (f, t2) ++ s2b) cova2)))));
+    clear hyp2; intros hyp2.
+  repeat (autodimp hyp2 h); exrepnd.
+
+  {
+    (* hyps_functionality *)
+
+    apply hyps_functionality_snoc2; simpl; auto;[].
+    introv equ sim; GC; lsubst_tac.
+
+    apply equality_in_member in equ.
+    exrepnd; computes_to_value_isvalue.
+
+    assert (equality lib (lsubstc a wa (snoc s1a0 (f, t1) ++ s1b) cova1)
+                     (lsubstc a wa s' c4)
+                     (lsubstc A w1 s1a0 c1)) as eqa.
+    {
+      vr_seq_true in hyp1.
+      generalize (hyp1 (snoc s1a0 (f, t1) ++ s1b) s'); clear hyp1; intros hyp1.
+      repeat (autodimp hyp1 h); exrepnd.
+      lsubst_tac.
+      allapply @member_if_inhabited.
+      apply tequality_mkc_member_implies_equality in hyp0; auto.
+    }
+
+    apply implies_tequality_mkc_member_if_member.
+
+    {
+      duplicate sim as sim'.
+      apply eqh in sim'.
+      rw @eq_hyps_app in sim'; simpl in sim'; exrepnd; subst; cpx.
+      apply app_split in sim'0; repnd; allrw length_snoc;
+        try (complete (allrw; sp)); subst; cpx.
+
+      assert (disjoint (remove_nvars [x] (free_vars B)) (dom_csub s1b0)) as disj1.
+      {
+        apply similarity_dom in sim1; repnd.
+        rw sim7.
+        rewrite vars_hyps_substitute_hyps; auto.
+      }
+
+      assert (disjoint (remove_nvars [x] (free_vars B)) (dom_csub s2b0)) as disj2.
+      {
+        apply sub_eq_hyps_dom in sim'1; repnd.
+        rw sim'1; auto.
+      }
+
+      rw @eq_hyps_snoc in sim'5; simpl in sim'5; exrepnd; subst; cpx.
+      lsubst_tac.
+
+      vr_seq_true in hyp1.
+      pose proof (hyp1 (snoc s1a (f, t0) ++ s1b0) (snoc s2a1 (f, t3) ++ s2b0)) as h1h.
+      repeat (autodimp h1h h); exrepnd;[].
+      lsubst_tac.
+
+      pose proof (hyp1 (snoc s2a1 (f, t3) ++ s2b0) (snoc s2a1 (f, t3) ++ s2b0)) as h2h.
+      repeat (autodimp h2h h); exrepnd; eauto 3 with slow.
+      { eapply similarity_hyps_functionality_trans; eauto. }
+      { eapply similarity_refl; apply similarity_sym; eauto. }
+      clear h2h0.
+      lsubst_tac.
+
+      clear hyp1.
+
+      apply member_if_inhabited in h1h1.
+      apply member_if_inhabited in h2h1.
+
+      applydup @tequality_implies_if_member in h1h0; auto;[].
+
+      repeat (lsubstc_subst_aeq2;[]).
+      repeat (substc_lsubstc_vars3;[]).
+      repeat (lsubstc_weak;[]).
+
+      revert sim'0 h1h2; introv teqF teqA.
+
+(*Definition LEM_Type := forall T : Type, T + !T.*)
+
+Lemma tequality_function_implies_tequality_codomain {o} :
+  forall lib (A : @CTerm o) v1 v2 B1 B2 a1 a2 f,
+    (*LEM_Type
+    ->*) member lib f (mkc_function A v1 B1)
+    -> tequality lib (mkc_function A v1 B1) (mkc_function A v2 B2)
+    -> equality lib a1 a2 A
+    -> tequality lib (substc a1 v1 B1) (substc a2 v2 B2).
+Proof.
+  introv (*lemt*) mem teqF eqa.
+
+  apply tequality_function in teqF; repnd.
+
+  apply tequality_iff_ext_eq; repnd; dands; eauto 3 with slow.
+  introv; split; intro h.
+
+  {
+    pose proof (teqF (mkc_lam x (if equality lib (mkc_var x)
+
+  }
+
+Qed.
+
+XXXXXXXXXXXXXXX
+    }
+
+    vr_seq_true in hyp1.
+    generalize (hyp1 (snoc s1a0 (f, t1) ++ s1b) s'); clear hyp1; intros hyp1.
+    repeat (autodimp hyp1 h); exrepnd.
+    lsubst_tac.
+    allapply @member_if_inhabited.
+    rw @tequality_mkc_member_sp in hyp0; repnd.
+
+    assert (equality lib (lsubstc a wa (snoc s1a0 (f, t1) ++ s1b) c3)
+                     (lsubstc a wa s' c5)
+                     (lsubstc A w1 s1a0 c1)) as eqa.
+    {
+      sp.
+      unfold member in hyp1.
+      spcast; apply @equality_respects_cequivc_right with (t2 := lsubstc a wa (snoc s1a0 (f, t1) ++ s1b) c3); sp.
+    }
+
+    applydup sim5 in eqa.
+
+    duplicate sim as sim'.
+    apply eqh in sim'.
+
+    rw @eq_hyps_app in sim'; simpl in sim'; exrepnd; subst; cpx.
+    apply app_split in sim'0; repnd; allrw length_snoc;
+    try (complete (allrw; sp)); subst; cpx.
+
+    rw @eq_hyps_snoc in sim'5; simpl in sim'5; exrepnd; subst; cpx.
+    lsubst_tac.
+    rw @tequality_function in sim'0; repnd.
+
+    applydup sim'0 in eqa as teq.
+
+    assert (disjoint (remove_nvars [x] (free_vars B)) (dom_csub s1b0)) as disj1.
+    {
+      apply similarity_dom in sim1; repnd.
+      rw sim7.
+      rewrite vars_hyps_substitute_hyps; auto.
+    }
+
+    assert (disjoint (remove_nvars [x] (free_vars B)) (dom_csub s2b0)) as disj2.
+    {
+      apply sub_eq_hyps_dom in sim'1; repnd.
+      rw sim'1; auto.
+    }
+
+    repeat (substc_lsubstc_vars3;[]).
+
+    dands.
+
+    {
+      repeat (lsubstc_subst_aeq2;[]).
+      repeat (substc_lsubstc_vars3;[]).
+      repeat (lsubstc_weak;[]).
+      proof_irr.
+      auto.
+    }
+
+    rw @similarity_app in sim; simpl in sim; exrepnd; subst; cpx.
+    apply app_split in sim7; repnd; allrw length_snoc;
+    try (complete (allrw; sp)); subst; cpx.
+    apply app_split in sim9; repnd; allrw length_snoc;
+    try (complete (allrw; sp)); subst; cpx.
+    rw @similarity_snoc in sim12; simpl in sim12; exrepnd; subst; cpx.
+    lsubst_tac.
+    rw @equality_in_function in sim9; repnd.
+    applydup sim9 in eqa as eqf.
+
+    left.
+    repeat (lsubstc_subst_aeq2;[]).
+    repeat (substc_lsubstc_vars3;[]).
+    repeat (lsubstc_weak;[]).
+    proof_irr.
+    auto.
+  }
+
+
+  {
+    (* similarity *)
+
+    assert (wf_term (mk_member (mk_apply (mk_var f) a) (subst B x a))) as wm.
+    {
+      apply wf_member; sp; try (apply wf_apply; sp).
+      apply subst_preserves_wf_term; sp.
+    }
+
+    assert (cover_vars (mk_member (mk_apply (mk_var f) a) (subst B x a))
+                       (snoc s1a0 (f, t1) ++ s1b)) as cm.
+    {
+      apply cover_vars_member; sp.
+      apply cover_vars_apply; sp.
+      apply cover_vars_var.
+      rw @dom_csub_app; rw @dom_csub_snoc; rw in_app_iff; rw in_snoc; simpl; sp.
+      rw @cover_vars_eq; rw @dom_csub_app; rw @dom_csub_snoc; insub.
+      (* begin proof of last cover_vars *)
+      rw @cover_vars_eq; rw @cover_vars_covered; apply covered_subst; sp.
+      rw @dom_csub_app; rw @dom_csub_snoc; simpl.
+      rw cons_app; apply covered_app_weak_l.
+      clear sim2 sim5; unfold cover_vars_upto in c2; unfold covered.
+      prove_subvars c2; allsimpl; sp.
+      rw @dom_csub_csub_filter in l; rw in_remove_nvars in l; rw in_single_iff in l.
+      rw in_snoc; sp.
+      clear hyp1; rw @covered_equality in ct0; repnd.
+      unfold covered; unfold covered in ct1.
+      rw @vars_hyps_app in ct1; rw @vars_hyps_snoc in ct1; simpl in ct1.
+      rw @dom_csub_app; rw @dom_csub_snoc; simpl.
+      allapply @similarity_dom; repnd; allrw; rw @vars_hyps_substitute_hyps; sp.
+      (* end proof of last cover_vars *)
+    }
+
+    sim_snoc.
+    dands; auto.
+    lsubst_tac.
+    rw @member_eq.
+    rw <- @member_member_iff.
+
+    vr_seq_true in hyp1.
+    generalize (hyp1 (snoc s1a0 (f, t1) ++ s1b)
+                     (snoc s2a0 (f, t2) ++ s2b));
+      clear hyp1; intros hyp1.
+    repeat (autodimp hyp1 h); exrepnd.
+    lsubst_tac.
+    allapply @member_if_inhabited.
+    rw @tequality_mkc_member_sp in hyp0; repnd.
+    unfold member in hyp1.
+    apply sim2 in hyp1.
+
+    assert (disjoint (remove_nvars [x] (free_vars B)) (dom_csub s1b)) as disj1.
+    {
+      apply similarity_dom in sim1; repnd.
+      rw sim7.
+      rewrite vars_hyps_substitute_hyps; auto.
+    }
+
+    apply equality_refl in hyp1.
+    unfold member in *.
+    repeat (lsubstc_subst_aeq2;[]).
+    repeat (substc_lsubstc_vars3;[]).
+    repeat (lsubstc_weak;[]).
+    proof_irr.
+    auto.
+  }
+
+  (* conclusion *)
+
+  lsubst_tac; sp.
+
+  assert (wf_term (@mk_axiom p)) as wfax by eauto 2 with slow.
+
+  repeat (lsubstc_subst_aeq2;[]).
+  allrw @lsubstc_mk_axiom.
+  repeat (substc_lsubstc_vars3;[]).
+  proof_irr.
+
+  pose proof (lsubstc_snoc_move
+                e
+                (snoc s1a0 (f, t1) ++ s1b)
+                []
+                z
+                mkc_axiom
+                wfce) as xx1.
+  allrw app_nil_r.
+  allrw @dom_csub_app.
+  allrw @dom_csub_snoc.
+  allsimpl.
+  pose proof (xx1 pt0) as xx2; clear xx1.
+  autodimp xx2 hyp.
+  { apply similarity_dom in sim6; repnd.
+    rewrite sim7.
+    apply similarity_dom in sim1; repnd.
+    rewrite sim8.
+    rewrite vars_hyps_substitute_hyps; auto.
+    rw in_app_iff; rw in_snoc; intro i; repndors; tcsp.
+  }
+  exrepnd.
+  proof_irr.
+  rewrite <- xx0; clear xx0.
+
+  pose proof (lsubstc_snoc_move
+                e
+                (snoc s2a0 (f, t2) ++ s2b)
+                []
+                z
+                mkc_axiom
+                wfce) as xx1.
+  allrw app_nil_r.
+  allrw @dom_csub_app.
+  allrw @dom_csub_snoc.
+  allsimpl.
+  pose proof (xx1 pt3) as xx2; clear xx1.
+  autodimp xx2 hyp.
+  { apply similarity_dom in sim6; repnd.
+    rewrite sim6.
+    apply similarity_dom in sim1; repnd.
+    rewrite sim1.
+    rewrite vars_hyps_substitute_hyps; auto.
+    rw in_app_iff; rw in_snoc; intro i; repndors; tcsp.
+  }
+  exrepnd.
+  proof_irr.
+  rewrite <- xx0; clear xx0.
+
+  auto.
+Qed.
+
+(* begin hide *)
+
+Lemma rule_function_elimination_true {p} :
+  forall lib (A B C a e : NTerm) ea,
+  forall f x z : NVar,
+  forall H J : @barehypotheses p,
+    rule_true lib (rule_function_elimination
+                     A B C a e
+                     ea
+                     f x z
+                     H J).
+Proof.
+  introv.
+  apply rule_true3_implies_rule_true.
+  apply rule_function_elimination_true3.
+Qed.
+
+Lemma rule_function_elimination_true2 {o} :
+  forall lib A B C a e ea f x z H J,
+    @rule_true2 o lib (rule_function_elimination A B C a e ea f x z H J).
+Proof.
+  intros.
+  apply rule_true_iff_rule_true2.
+  apply rule_function_elimination_true.
+Qed.
+
+Lemma rule_function_elimination_true_ex {p} :
+  forall lib (A B C a e : NTerm) ea,
+  forall f x z : NVar,
+  forall H J : @barehypotheses p,
+    rule_true_if lib (rule_function_elimination
+                        A B C a e
+                        ea
+                        f x z
+                        H J).
+Proof.
+  intros.
+  generalize (rule_function_elimination_true lib A B C a e ea f x z H J); intro rt.
+  rw <- @rule_true_eq_ex in rt.
+  unfold rule_true_ex in rt; sp.
+Qed.
+
+Lemma rule_function_elimination_wf {o} :
+  forall (A B C a e : @NTerm o) ea f x z H J,
+    wf_term a
+    -> covered a (snoc (vars_hyps H) f ++ vars_hyps J)
+    -> !LIn z (vars_hyps H)
+    -> !LIn z (vars_hyps J)
+    -> z <> f
+    -> wf_term ea
+    -> wf_rule (rule_function_elimination A B C a e ea f x z H J).
+Proof.
+  introv wa cov nizH nizJ dzf wea.
+
+  introv pwf m; allsimpl; repdors; subst; sp;
+  allunfold @pwf_sequent; wfseq; sp.
+
+  {
+    allrw @vswf_hypotheses_nil_eq.
+    allrw @wf_hypotheses_app; repnd.
+    allrw @wf_hypotheses_snoc; repnd.
+    allsimpl.
+    allapply @isprog_vars_implies_wf.
+    allrw <- @wf_function_iff; tcsp.
+  }
+
+  {
+    allrw @vswf_hypotheses_nil_eq.
+    allrw @wf_hypotheses_app; repnd.
+    allrw @wf_hypotheses_snoc; repnd.
+    allsimpl.
+    allapply @isprog_vars_implies_covered.
+    allrw @covered_function; repnd.
+    apply covered_snoc_app_weak.
+    apply covered_app_weak_l; auto.
+  }
+
+  {
+    allrw @vswf_hypotheses_nil_eq.
+    rw @wf_hypotheses_snoc; simpl; dands; tcsp.
+    - apply isprog_vars_member; dands.
+      + apply isprog_vars_apply; dands.
+        * apply isprog_vars_var_iff.
+          rw @vars_hyps_app.
+          rw @vars_hyps_snoc; simpl.
+          rw in_app_iff.
+          rw in_snoc; tcsp.
+        * rw @isprog_vars_iff_covered; dands; auto.
+          rw @vars_hyps_app.
+          rw @vars_hyps_snoc; simpl; auto.
+      + apply isprog_vars_subst2; auto.
+        * allrw @wf_hypotheses_app; repnd.
+          allrw @wf_hypotheses_snoc; repnd.
+          allsimpl.
+          allapply @isprog_vars_implies_wf.
+          allrw <- @wf_function_iff; tcsp.
+        * rw @isprog_vars_iff_covered; dands; auto.
+          rw @vars_hyps_app.
+          rw @vars_hyps_snoc; simpl; auto.
+        * allrw @wf_hypotheses_app; repnd.
+          allrw @wf_hypotheses_snoc; repnd.
+          allsimpl.
+          allrw <- @isprog_vars_function_iff; repnd.
+          allrw @vars_hyps_app.
+          allrw @vars_hyps_snoc; simpl.
+          eapply isprog_vars_subvars;[|eauto].
+          rw subvars_eq; introv i; allsimpl.
+          allrw in_app_iff; allrw in_snoc; tcsp.
+    - intro i.
+      allrw @vars_hyps_app.
+      allrw @vars_hyps_snoc; allsimpl.
+      allrw in_app_iff; allrw in_snoc.
+      repndors; tcsp.
+  }
+
+  {
+    allrw @wf_term_eq.
+    allrw @nt_wf_lsubst_iff; tcsp.
+  }
+
+  {
+    apply covered_snoc_weak; auto.
+  }
+Qed.
+
+Lemma rule_function_elimination_wf2 {o} :
+  forall (A B C a e : @NTerm o) ea f x z H J,
+    wf_term a
+    -> covered a (snoc (vars_hyps H) f ++ vars_hyps J)
+    -> !LIn z (vars_hyps H)
+    -> !LIn z (vars_hyps J)
+    -> z <> f
+    -> wf_rule2 (rule_function_elimination A B C a e ea f x z H J).
+Proof.
+  introv wa cova nizH nizJ dzf wf j.
+  allsimpl; repndors; subst; tcsp;
+  allunfold @wf_bseq; repnd; allsimpl; wfseq.
+
+  - allrw @vswf_hypotheses_nil_eq.
+    allrw @wf_hypotheses_app; repnd.
+    allrw @wf_hypotheses_snoc; repnd.
+    allapply @isprog_vars_implies_wf.
+    allrw <- @wf_function_iff; tcsp.
+
+  - allrw @vswf_hypotheses_nil_eq.
+    allrw @wf_hypotheses_app; repnd.
+    allrw @wf_hypotheses_snoc; repnd.
+    allapply @isprog_vars_implies_covered.
+    allrw @covered_function; repnd.
+    apply covered_snoc_app_weak.
+    apply covered_app_weak_l; auto.
+
+  - allrw @vswf_hypotheses_nil_eq.
+    rw @wf_hypotheses_snoc; simpl; dands; tcsp.
+    { apply isprog_vars_member; dands.
+      + apply isprog_vars_apply; dands.
+        * apply isprog_vars_var_iff.
+          rw @vars_hyps_app.
+          rw @vars_hyps_snoc; simpl.
+          rw in_app_iff.
+          rw in_snoc; tcsp.
+        * rw @isprog_vars_iff_covered; dands; auto.
+          rw @vars_hyps_app.
+          rw @vars_hyps_snoc; simpl; auto.
+      + apply isprog_vars_subst2; auto.
+        * allrw @wf_hypotheses_app; repnd.
+          allrw @wf_hypotheses_snoc; repnd.
+          allsimpl.
+          allapply @isprog_vars_implies_wf.
+          allrw <- @wf_function_iff; tcsp.
+        * rw @isprog_vars_iff_covered; dands; auto.
+          rw @vars_hyps_app.
+          rw @vars_hyps_snoc; simpl; auto.
+        * allrw @wf_hypotheses_app; repnd.
+          allrw @wf_hypotheses_snoc; repnd.
+          allsimpl.
+          allrw <- @isprog_vars_function_iff; repnd.
+          allrw @vars_hyps_app.
+          allrw @vars_hyps_snoc; simpl.
+          eapply isprog_vars_subvars;[|eauto].
+          rw subvars_eq; introv i; allsimpl.
+          allrw in_app_iff; allrw in_snoc; tcsp.
+    }
+    { intro i.
+      allrw @vars_hyps_app.
+      allrw @vars_hyps_snoc; allsimpl.
+      allrw in_app_iff; allrw in_snoc.
+      repndors; tcsp.
+    }
+
+  - apply covered_snoc_weak; auto.
+Qed.
+
+
+
+
+
+(* end hide *)
+
+(**
+
+  The Nuprl manual%~\cite{Kreitz:02}% presents various useful rules to
+  reason about function types.  This section prove the truth of
+  several of these rules.
+
+*)
+
+
+
+
+(* end hide *)
